theories/CTree/Logic/AF.v
@@ -11,11 +11,13 @@ From CTree Require Import
   Events.WriterE
   CTree.Core
   CTree.Equ
+  CTree.SBisim
   CTree.Interp.Core
   CTree.Interp.State
   CTree.Logic.Trans
   CTree.Logic.CanStep
   Logic.Ctl
+  Logic.AX
   Logic.Kripke
   Logic.Setoid.
 
@@ -30,7 +32,7 @@ Local Open Scope ctree_scope.
 Section BasicLemmas.
   Context {E: Type} {HE: Encode E} {X: Type}.
 
-  Lemma done_af: forall (t: ctree E X) φ w,
+  Lemma af_done: forall (t: ctree E X) φ w,
       is_done w ->
       <( t, w |= AF now φ )> ->
       φ w.
@@ -41,6 +43,18 @@ Section BasicLemmas.
     - destruct H0 as ((? & ? & ?) & ?).
       exfalso.
       eapply done_not_ktrans with (t:=t); eauto.
+  Qed.
+
+  Lemma af_stuck: forall w φ,
+      <( {Ctree.stuck: ctree E X}, w |= AF φ )> <->
+      <( {Ctree.stuck: ctree E X}, w |= φ )>.
+  Proof.
+    split; intros.
+    - cbn in H; dependent induction H; auto.
+      destruct H0, H1.
+      apply can_step_stuck in H1.
+      contradiction.
+    - now next; left.
   Qed.
 
   Lemma af_ret: forall r w (Rr: rel X (World E)),      
@@ -62,40 +76,37 @@ Section BasicLemmas.
         rewrite ctl_done.
         now constructor.       
   Qed.
-  Hint Resolve af_ret: ctl.
 
-
-  Lemma af_tau: forall (t: ctree E X) w φ,
-      <( t, w |= AF φ )> -> 
-      <( {Tau t}, w |= AF φ )>.
-  Proof.
-    intros.
-  Admitted.
-
-  Lemma afax_tau: forall (t: ctree E X) w φ,
-      <( t, w |= AF AX now φ )> -> 
-      <( {Tau t}, w |= AF AX (now φ) )>.
-  Proof.
-    intros.
-    Transparent entailsF.
-    unfold entailsF in H.
-    induction H.
+  Lemma not_done_vis_af: forall (t: ctree E X) φ w,
+      <( t, w |= AF vis φ )> ->
+      not_done w.
+  Proof with eauto with ctl.
+    intros * Hf.
+    next in Hf ; destruct Hf.
+    - rewrite ctl_vis in H; inv H...
     - destruct H.
-      next; left. 
-      split.
-      + now apply can_step_tau.
-      + intros *  TR.
-        rewrite ktrans_tau in TR.
-        now apply H0 with t'.
-    - destruct H0, H1; clear H H1.
-      next; right.
-      split.
-      + now apply can_step_tau.
-      + intros * TR.
-        rewrite ktrans_tau in TR.
-        now apply H2.
+      now apply can_step_not_done with t.
   Qed.
-  
+
+  Lemma not_done_pure_af: forall (t: ctree E X) w,
+      <( t, w |= AF pure )> ->
+      not_done w.
+  Proof with eauto with ctl.
+    intros * Hf.
+    next in Hf ; destruct Hf.
+    - rewrite ctl_pure in H; subst...
+    - destruct H.
+      now apply can_step_not_done with t.
+  Qed.
+
+  Lemma af_guard: forall (t: ctree E X) w φ,
+      <( {Guard t}, w |= AF φ )> <->
+      <( t, w |= AF φ )>.
+  Proof.
+    intros.
+    now rewrite sb_guard.
+  Qed.
+
   Lemma af_br: forall n (k: fin' n -> ctree E X) w φ,
       <( {Br n k}, w |= AF now φ )> <->
         (forall (i: fin' n), <( {k i}, w |= AF now φ )>).
@@ -116,7 +127,7 @@ Section BasicLemmas.
         * intros t' w' TR'.
           apply ktrans_br in TR' as (? & -> & -> & ?).
           apply H.
-      + apply done_af with (φ:=φ) (t:= k Fin.F1) in i; auto.
+      + apply af_done with (φ:=φ) (t:= k Fin.F1) in i; auto.
         next; left.
         now apply ctl_now.
   Qed.
@@ -136,225 +147,31 @@ Section BasicLemmas.
         now rewrite <- H0.
   Qed.
 
+  Lemma af_ret_inv: forall (x: X) w R,
+      <( {Ret x}, w |= AF (AX done R) )> ->
+      R x w.
+  Proof.
+    intros.
+    next in H; destruct H.
+    - destruct H.
+      destruct H as (tstuck & w' & TR).
+      specialize (H0 _ _ TR).
+      inv TR; cbn in H0; now dependent destruction H0.
+    - next in H; destruct H.
+      destruct H as (tstuck & w' & TR).
+      specialize (H0 _ _ TR).
+      inv TR; observe_equ H1; rewrite <- Eqt, H3 in H0.
+      + rewrite af_stuck in H0.
+        apply ax_stuck in H0.
+        rewrite ctl_done in H0.
+        now dependent destruction H0.
+      + rewrite af_stuck in H0.
+        apply ax_stuck in H0.
+        cbn in H0.
+        now dependent destruction H0.
+  Qed.
+
 End BasicLemmas.
-
-Section AfIndLemma.
-  Context {E: Type} {HE: Encode E} {X: Type}.
-  
-  (*| [t |= AF φ] is semantic and requires double induction, on [AF] and inside it, in
-    [ktrans]. Attempt to simplify to one induction with [AFInd] |*)
-  Inductive AFInd(φ: ctree E X -> World E -> Prop): ctree E X -> World E -> Prop :=
-  | AFIndBase: forall (t: ctree E X) (w: World E),
-      φ t w ->
-      AFInd φ t w
-  | AFIndDoneBase: forall t (x: X),
-      observe t = RetF x ->
-      φ Ctree.stuck (Done x) ->
-      AFInd φ t Pure
-  | AFIndFinishBase: forall t (e: E) (v: encode e) (x: X),
-      observe t = RetF x ->
-      φ Ctree.stuck (Finish e v x) ->
-      AFInd φ t (Obs e v)
-  | AFIndTau: forall t u w,
-      observe t = TauF u ->
-      AFInd φ u w ->
-      AFInd φ t w
-  |AFIndVis: forall (t: ctree E X) w e k (_: encode e),
-      observe t = VisF e k ->
-      not_done w ->
-      (forall (v: encode e), AFInd φ (k v) (Obs e v)) ->
-      AFInd φ t w
-  |AFIndBr: forall n (t: ctree E X) w k,
-      observe t = BrF n k ->
-      not_done w ->
-      (forall (i: fin' n), AFInd φ (k i) w) ->
-      AFInd φ t w.
-
-  Global Instance proper_equ_afind φ {HP: Proper (equ eq ==> eq ==> iff) φ}:
-    Proper (equ eq ==> eq ==> iff) (AFInd φ).
-  Proof.
-    unfold Proper, respectful.
-    intros; subst; split; intros Hind.
-    - generalize dependent y.
-      induction Hind; intros.
-      + apply AFIndBase; auto.
-        now rewrite <- H0.
-      + apply AFIndDoneBase with x; auto.
-        unfold equ in H1; step in H1; cbn in H1; dependent destruction H1; congruence.
-      + apply AFIndFinishBase with x; auto.
-        unfold equ in H1; step in H1; cbn in H1; dependent destruction H1; congruence.
-      + unfold equ; step in H0; cbn in H0; rewrite H in H0.
-        dependent destruction H0.
-        apply IHHind in H0.
-        apply AFIndTau with t2; congruence.
-      + unfold equ; step in H3; cbn in H3; rewrite H in H3.
-        dependent destruction H3.
-        eapply AFIndVis with e k2; auto.
-        intros.
-        apply H2, H3.
-      + unfold equ; step in H3; cbn in H3; rewrite H in H3.
-        dependent destruction H3.
-        eapply AFIndBr; eauto. 
-        intros.
-        eapply H2 with i, H3.
-    - generalize dependent x.
-      induction Hind; intros.
-      + apply AFIndBase; auto.
-        now rewrite H0.
-      + apply AFIndDoneBase with x; auto.
-        unfold equ in H1; step in H1; cbn in H1; dependent destruction H1; congruence.
-      + apply AFIndFinishBase with x; auto.
-        unfold equ in H1; step in H1; cbn in H1; dependent destruction H1; congruence.
-      + unfold equ; step in H0; cbn in H0; rewrite H in H0.
-        dependent destruction H0.
-        apply IHHind in H0.
-        apply AFIndTau with t1; congruence.
-      + unfold equ; step in H3; cbn in H3; rewrite H in H3.
-        dependent destruction H3.
-        eapply AFIndVis with e k1; auto.
-        intros.
-        apply H2, H3.
-      + unfold equ; step in H3; cbn in H3; rewrite H in H3.
-        dependent destruction H3.
-        eapply AFIndBr; eauto. 
-        intros.
-        eapply H2 with i, H3.
-  Qed.  
-
-  Lemma af_ind_stuck_done: forall (x: X) φ,
-    AFInd φ Ctree.stuck (Done x) <->
-    φ Ctree.stuck (Done x).
-  Proof.
-    split; intros.
-    - dependent induction H; auto.
-    - now apply AFIndBase.
-  Qed.
-
-  Lemma af_ind_stuck_finish: forall (e: E) (v: encode e) (x: X) φ,
-    AFInd φ Ctree.stuck (Finish e v x) <->
-    φ Ctree.stuck (Finish e v x).
-  Proof.
-    split; intros.
-    - dependent induction H; auto.
-    - now apply AFIndBase.
-  Qed.
-
-  (* This is a super useful lemma, it allows us to do induction on [AFInd]
-     instead of two inductions on [cau] and [trans] *)
-  Opaque Ctree.stuck.
-  Lemma af_afind : forall (t: ctree E X) (w: World E) φ,
-       cau true (fun _ _ => True) φ t w -> AFInd φ t w.
-  Proof.
-    intros; induction H.
-    - now apply AFIndBase.
-    - destruct H0, H1; clear H H1.
-      destruct H0 as (t' & w' & TR).
-      cbn in TR.
-      dependent induction TR.
-       + eapply AFIndTau with (u:=t0); auto.
-        eapply IHTR with (t':=t'); auto.
-        -- intros t_ w_ TR_.
-           apply H2; cbn.
-           rewrite <- x0.
-           now apply ktrans_tau.
-        -- intros t_ w_ TR_.
-           apply H3; cbn.
-           rewrite <- x0.
-           now apply ktrans_tau.
-       + observe_equ x.
-         eapply AFIndBr with (n:=n) (k:=k); auto.
-         intros j.
-         apply H3; cbn.
-         rewrite <- x0.
-         apply KtransBr with j; auto.
-       + observe_equ x.
-         eapply AFIndVis with (e:=e) (k:=k); auto.
-         intros v'.
-         apply H3; cbn.
-         rewrite <- x0.
-         apply KtransObs; auto.     
-       + apply AFIndDoneBase with (x:=x0); auto.
-         assert (TR_: [t, Pure] ↦ [Ctree.stuck, Done x0]).
-         { cbn; rewrite <- x1; apply KtransDone; auto. }
-         specialize (H3 _ _ TR_).
-         now apply af_ind_stuck_done.
-       + apply AFIndFinishBase with (x:=x0); auto.
-         assert (TR_: [t, Obs e v] ↦ [Ctree.stuck, Finish e v x0]).
-         { cbn; rewrite <- x1; apply KtransFinish; auto. }
-         specialize (H3 _ _ TR_).
-         now apply af_ind_stuck_finish.
-  Qed.
-
-  (* -> *)
-  Lemma afind_af {Hpr: @Productive E HE} φ
-    {HP: Proper (equ eq ==> eq ==> iff) φ}
-    {TauInv: forall (t: ctree E X) w, φ t w  -> φ (Tau t) w}
-    : forall (t: ctree E X) (w: World E),
-      AFInd φ t w -> cau true (fun _ _ => True) φ t w.
-  Proof.
-    intros; induction H.
-    - now apply MatchA.
-    - apply StepA; auto; split.
-      + exists Ctree.stuck, (Done x).
-        Opaque Ctree.stuck.
-        cbn. rewrite H.
-        apply KtransDone; auto.
-      + intros t' w' TR.
-        cbn in TR.        
-        dependent induction TR.
-        * rewrite H in x1; inv x1.
-        * rewrite H in x1; inv x1.
-        * rewrite H in x1; inv x1.
-        * observe_equ x.
-          rewrite <- Eqt, H1.
-          rewrite <- x2 in H.
-          inv H.
-          now apply MatchA.
-    - apply StepA; auto; split.
-      + exists Ctree.stuck, (Finish e v x).
-        Opaque Ctree.stuck.
-        cbn. rewrite H.
-        apply KtransFinish; auto.
-      + intros t' w' TR.
-        cbn in TR.
-        dependent induction TR.
-        * rewrite H in x1; inv x1.
-        * rewrite H in x1; inv x1.
-        * rewrite H in x1; inv x1.
-        * observe_equ x.
-          rewrite <- Eqt, H1.
-          rewrite <- x2 in H.
-          inv H.
-          now apply MatchA.
-    - observe_equ H.
-      rewrite Eqt; clear Eqt.
-      destruct IHAFInd.
-      + apply MatchA.
-        (* TauInv here *)
-        now apply TauInv.
-      + destruct H2.
-        apply StepA; auto.
-        split.
-        * now apply can_step_tau.
-        * intros t' w' TR.
-          apply H3.
-          now rewrite ktrans_tau in TR.
-    - observe_equ H.
-      rewrite Eqt; clear Eqt.
-      apply StepA; auto; split.
-      + now apply can_step_vis.
-      + intros t' w' TR.
-        apply ktrans_vis in TR as (v & -> & <- & ?).
-        eapply H2.
-    - observe_equ H.
-      rewrite Eqt; clear Eqt.
-      apply StepA; auto; split.
-      + now apply can_step_br.
-      + intros t' w' TR.
-        apply ktrans_br in TR as (v & -> & <- & ?).
-        eapply H2.
-  Qed.
-End AfIndLemma.
 
 Section AfDoneIndLemma.
   Context {E: Type} {HE: Encode E} {X: Type}
@@ -370,8 +187,8 @@ Section AfDoneIndLemma.
       observe t = RetF x ->
       φ x (Obs e v) ->
       AFDoneInd t (Obs e v)
-  | AFDoneIndTau: forall t u w,
-      observe t = TauF u ->
+  | AFDoneIndGuard: forall t u w,
+      observe t = GuardF u ->
       AFDoneInd u w ->
       AFDoneInd t w
   |AFDoneIndVis: forall (t: ctree E X) w e k (_: encode e),
@@ -404,7 +221,7 @@ Section AfDoneIndLemma.
       + unfold equ; step in H0; cbn in H0; rewrite H in H0.
         dependent destruction H0.
         apply IHHind in H0.
-        apply AFDoneIndTau with t2; congruence.
+        apply AFDoneIndGuard with t2; congruence.
       + unfold equ; step in H3; cbn in H3; rewrite H in H3.
         dependent destruction H3.
         eapply AFDoneIndVis with e k2; auto; intros.
@@ -427,7 +244,7 @@ Section AfDoneIndLemma.
       + unfold equ; step in H0; cbn in H0; rewrite H in H0.
         dependent destruction H0.
         apply IHHind in H0.
-        apply AFDoneIndTau with t1; congruence.
+        apply AFDoneIndGuard with t1; congruence.
       + unfold equ; step in H3; cbn in H3; rewrite H in H3.
         dependent destruction H3.
         eapply AFDoneIndVis with e k1; auto; intros.
@@ -448,19 +265,18 @@ Section AfDoneIndLemma.
   Lemma afdone_ind: forall (t: ctree E X) w,
       <( t, w |= AF AX done φ )> ->
       AFDoneInd t w.
-  Proof.
+  Proof with eauto with ctl.
     intros; induction H.
     - next in H.
       destruct H as [(t' & w' & TR) H].
       cbn in TR.
       dependent induction TR.
-      + eapply AFDoneIndTau with (u:=t0); auto.
-        eapply IHTR; auto.
+      + eapply AFDoneIndGuard with (u:=t0); auto.
+        eapply IHTR...
         intros t_ w_ TR_.
         apply H; cbn.
-        rewrite <- x0.
-        now apply ktrans_tau.
-      + eapply AFDoneIndBr; eauto.
+        rewrite <- x0... 
+      + eapply AFDoneIndBr...
         intros v'.
         assert (TR: ktrans_ (observe t) w (observe (k v')) w).
         { rewrite <- x0; apply ktrans_br; exists v'; eauto. }
@@ -490,16 +306,16 @@ Section AfDoneIndLemma.
        destruct H0 as (t' & w' & TR).
        cbn in TR.
        dependent induction TR.
-       + eapply AFDoneIndTau with (u:=t0); auto.
+       + eapply AFDoneIndGuard with (u:=t0); auto.
         eapply (IHTR) with (t':=t'); auto.
         -- intros t_ w_ TR_.
            apply H2; cbn.
            rewrite <- x0.
-           now apply ktrans_tau.
+           now apply ktrans_guard.
         -- intros t_ w_ TR_.
            apply H3; cbn.
            rewrite <- x0.
-           now apply ktrans_tau.
+           now apply ktrans_guard.
        + observe_equ x.
          eapply AFDoneIndBr with n k; auto.
          intros i'.
@@ -524,42 +340,10 @@ Section AfDoneIndLemma.
         now apply afdoneind_stuck in H3.
   Qed.
 
-  Lemma af_ret_inv: forall (x: X) w R,
-      <( {Ret x}, w |= AF (AX done R) )> ->
-      R x w.
-  Proof.
-    intros.
-    apply af_afind in H.
-    dependent induction H.
-    - destruct H.
-      destruct H as (t' & w' & TR).
-      specialize (H0 _ _ TR).
-      inv H0; destruct w; cbn in TR; dependent destruction TR; auto.
-    - destruct H0.
-      apply can_step_not_done in H.
-      inv H.
-    - destruct H0.
-      apply can_step_not_done in H.
-      inv H.
-  Qed.
-
 End AfDoneIndLemma.
 
 Section CtlAfBind.
   Context {E: Type} {HE: Encode E}.
-
-  Lemma af_stuck{X}: forall φ w,
-      φ w <->
-      <( {Ctree.stuck: ctree E X}, w |= AF now φ )>.
-  Proof.
-    split; intros.
-    - next; left; auto.
-    - remember Ctree.stuck as S. 
-      apply af_afind in H.
-      Transparent Ctree.stuck.
-      induction H; subst; auto; cbn in *;
-        dependent destruction H; auto.      
-  Qed.
 
   Typeclasses Transparent equ.
   Theorem af_bind_vis{X Y}: forall (t: ctree E Y) (k: Y -> ctree E X) φ w,
@@ -567,27 +351,31 @@ Section CtlAfBind.
       <( {x <- t ;; k x}, w |= AF vis φ )>.
   Proof.
     intros * Haf.
-    apply af_afind in Haf.
-    revert X k.    
-    induction Haf; intros; subst. 
-    - (* Base *)
-      next; left; cbn; apply H.
-    - (* Done *)
-      inv H0.
-    - (* Finish *)
-      inv H0.
-    - (* Tau *)
-      observe_equ H.
-      rewrite Eqt, bind_tau.
-      apply af_tau; eauto.
-    - (* Vis *)
-      observe_equ H.
-      rewrite Eqt, bind_vis.
-      apply af_vis; eauto.
-    - (* Br *)
-      observe_equ H.
-      rewrite Eqt, bind_br.
-      apply af_br; eauto.      
+    revert X k.
+    induction Haf; intros; subst.
+    - (* MatchA *)
+      next; left; cbn.
+      apply ctl_vis in H; inv H; now constructor.
+    - (* StepA *)
+      destruct H0, H1; clear H H0.      
+      next; right; next; split.
+      + (* can_step *)
+        destruct H1 as (t' & w' & TR').
+        eapply can_step_bind_l with t' w'; auto.
+        eapply not_done_vis_af with (t:=t').
+        now apply H2.
+      + (* AX AF *)
+        intros t_ w_ TR_.
+        apply ktrans_bind_inv in TR_ as
+            [(t' & TR' & Hd & ->) |
+              (x & w' & TR' & Hr & TRk)].
+        * now apply H3.
+        * specialize (H2 _ _ TR').
+          inv H2.
+          apply ctl_vis in H; inv H. 
+          -- inv Hr.
+          -- destruct H0.
+             now apply can_step_stuck in H0.
   Qed.
 
   Theorem af_bind_pure{X Y}: forall (t: ctree E Y) (k: Y -> ctree E X) w,
@@ -595,55 +383,31 @@ Section CtlAfBind.
       <( {x <- t ;; k x}, w |= AF pure )>.
   Proof.
     intros * Haf.
-    apply af_afind in Haf.
-    revert X k.    
-    induction Haf; intros; subst. 
-    - (* Base *)
-      next; left; now cbn. 
-    - (* Done *)
-      inv H0.
-    - (* Finish *)
-      inv H0.
-    - (* Tau *)
-      observe_equ H.
-      rewrite Eqt, bind_tau.
-      apply af_tau; eauto.
-    - (* Vis *)
-      observe_equ H.
-      rewrite Eqt, bind_vis.
-      apply af_vis; eauto.
-    - (* Br *)
-      observe_equ H.
-      rewrite Eqt, bind_br.
-      apply af_br; eauto.   
+    revert X k.
+    induction Haf; intros; subst.
+    - (* MatchA *)
+      next; left; cbn.
+      now apply ctl_pure in H. 
+    - (* StepA *)
+      destruct H0, H1; clear H H0.      
+      next; right; next; split.
+      + (* can_step *)
+        destruct H1 as (t' & w' & TR').
+        eapply can_step_bind_l with t' w'; auto.
+        eapply not_done_pure_af with (t:=t').
+        now apply H2.
+      + (* AX AF *)
+        intros t_ w_ TR_.
+        apply ktrans_bind_inv in TR_.
+        destruct TR_ as [(t' & TR' & Hd & ->) | (x & w' & TR' & Hr & TRk)].
+        * now apply H3.
+        * specialize (H2 _ _ TR').
+          inv H2.
+          apply ctl_pure in H; subst.
+          -- inv Hr.
+          -- destruct H0.
+             now apply can_step_stuck in H0.
   Qed.
-
-  Lemma can_step_bind_r{X Y}: forall (t: ctree E Y) (k: Y -> ctree E X) w R,      
-      <( t, w |= AF AX done R )> ->
-      (forall y w, R y w -> can_step (k y) w) ->
-      can_step (x <- t ;; k x) w.
-  Proof.    
-    intros.
-    apply afdone_ind in H.
-    generalize dependent k.
-    induction H; intros; observe_equ H; rewrite Eqt.
-    - (* Done x *)
-      rewrite bind_ret_l.
-      now apply H1.
-    - (* Finish *)
-      rewrite bind_ret_l.
-      now apply H1.
-    - (* Tau *)
-      rewrite bind_tau.
-      apply can_step_tau; eauto.
-    - (* Vis *)
-      rewrite bind_vis.
-      apply can_step_vis; auto.
-    - (* Br *)
-      rewrite bind_br.
-      apply can_step_br; auto.
-  Qed.
-  Hint Resolve can_step_bind_r: ctl.
 
   Theorem af_bind_r{X Y}: forall (t: ctree E Y) (k: Y -> ctree E X) w φ R,
       <( t, w |= AF AX done R )> ->
@@ -662,8 +426,8 @@ Section CtlAfBind.
     - (* Finish *)
       rewrite bind_ret_l; eauto with ctl.
     - (* Tau *)
-      rewrite bind_tau.
-      apply af_tau; eauto with ctl.
+      rewrite bind_guard.
+      apply af_guard; eauto with ctl.
     - (* Vis *)
       rewrite bind_vis.
       apply af_vis; eauto with ctl.
@@ -721,14 +485,15 @@ Section CtlAfIter.
     intros.
     unfold iter, MonadIter_ctree.
     rewrite unfold_iter.
-    eapply af_bind_r with (R:=fun (x : I + X) (w' : World E) =>
-                                match x with
-                                | inl i' => Ri i' w' /\ Rv (i', w') (i, w)
-                                | inr r' => Rr r' w'
-                                end); auto.
+    eapply af_bind_r with
+      (R:=fun (x : I + X) (w' : World E) =>
+            match x with
+            | inl i' => Ri i' w' /\ Rv (i', w') (i, w)
+            | inr r' => Rr r' w'
+            end); auto.
     intros [i' | r] w'.
     - intros (Hi' & Hv) Hd.
-      apply af_tau.
+      apply af_guard.
       remember (i', w') as y.
       replace i' with (fst y) by now subst.
       replace w' with (snd y) by now subst.      
@@ -768,7 +533,8 @@ Section CtlAfIter.
     <( {iter k i}, w |= AF done Rr )>.
   Proof.
     intros.
-    eapply af_iter_nat with (Ri:=fun _ => not_done) (f:=f); intros; auto.
+    eapply af_iter_nat with
+      (Ri:=fun _ => not_done) (f:=f); intros; auto.
   Qed.
 
   (* Well-founded induction on length of lists *)
@@ -785,7 +551,8 @@ Section CtlAfIter.
     <( {iter k i}, w |= AF done Rr )>.
   Proof.
     intros.
-    eapply af_iter_nat with Ri (fun i w => length (f i w)); auto.
+    eapply af_iter_nat with
+      Ri (fun i w => length (f i w)); auto.
   Qed.
 
   Lemma af_iter_list'{A X I} Rr (f: I -> World E -> list A) (i: I) w (k: I -> ctree E (I + X)):
@@ -802,9 +569,9 @@ Section CtlAfIter.
     <( {iter k i}, w |= AF done Rr )>.
   Proof.
     intros.
-    eapply af_iter_list with (Ri:=fun _ => not_done) (f:=f); intros; auto.
-  Qed.
-  
+    eapply af_iter_list with
+      (Ri:=fun _ => not_done) (f:=f); intros; auto.
+  Qed.  
 End CtlAfIter.
 
 (*| Combinators for [interp_state] |*)
@@ -847,11 +614,12 @@ Section CtlAfState.
     (forall (i: I) w s,
         Ri i w s ->
         <( {interp_state h (k i) s}, w |= AF AX done
-                                       {fun '(x, s') w' =>
-                                          match x with
-                                          | inl i' => Ri i' w' s' /\ Rv (i', w', s') (i, w, s)
-                                          | inr r' => Rr (r',s') w'
-                                          end})>) ->
+          {fun '(x, s') w' =>
+             match x with
+             | inl i' => Ri i' w' s'
+                        /\ Rv (i', w', s') (i, w, s)
+             | inr r' => Rr (r',s') w'
+             end})>) ->
     well_founded Rv ->
     Ri i w s ->
     <( {interp_state h (Ctree.iter k i) s}, w |= AF done Rr )>.
@@ -877,7 +645,7 @@ Section CtlAfState.
                       end); auto.
     intros ([i' | r] & s') w'; cbn.
     - intros (Hi' & Hv) Hd.
-      apply af_tau.
+      apply af_guard.
       remember (i', w',s') as y.
       replace i' with (fst (fst y)) by now subst.
       replace w' with (snd (fst y)) by now subst.
@@ -947,11 +715,11 @@ Section CtlAfStateList.
     (forall (i: I) w (l: list A),
         not_done w ->
         <( {interp_state h (k i) l}, w |= AF AX done
-                 {fun '(x, l') w' =>
-                    match (x: I + X) with
-                    | inl _ => not_done w' /\ length l' < length l
-                    | inr r' => Rr (r',l') w'
-                    end})>) ->
+             {fun '(x, l') w' =>
+                match (x: I + X) with
+                | inl _ => not_done w' /\ length l' < length l
+                | inr r' => Rr (r',l') w'
+                end})>) ->
     not_done w ->
     <( {interp_state h (Ctree.iter k i) l}, w |= AF done Rr )>.
   Proof.
