theories/CTree/Logic/Trans.v
@@ -15,6 +15,7 @@ From Coq Require Import
 From CTree Require Import
   CTree.Core
   CTree.Equ
+  CTree.Trans
   Utils.Trc
   CTree.Events.Writer
   Events.Core
@@ -29,14 +30,14 @@ Local Open Scope ctree_scope.
 Notation ctreeW W := (ctree (writerE W)).
 
 Section CTreeTrans.
-  Context {E: Type} `{HE: Encode E} {X: Type}.
+  Context {E: Type} `{HE: Encode E}.
   Notation encode := (@encode E HE).
 
   (*| Kripke transition system |*)
   Inductive ktrans_{X}: ctree' E X -> World E -> ctree' E X -> World E -> Prop :=
-  | KtransTau w w' (t t': ctree E X): 
+  | KtransGuard w w' (t t': ctree E X): 
     ktrans_ (observe t) w (observe t') w' ->
-    ktrans_ (TauF t) w (observe t') w'
+    ktrans_ (GuardF t) w (observe t') w'
   | KtransBr (n: nat) (i: fin' n) k t w:
     not_done w ->
     t ≅ k i ->
@@ -51,8 +52,9 @@ Section CTreeTrans.
   | KtransFinish (e: E) (v: encode e) (x: X) t:
     t ≅ Ctree.stuck ->
     ktrans_ (RetF x) (Obs e v) (observe t) (Finish e v x).
-
-  Global Instance ktrans_equ_aux1 (t: ctree' E X) (w: World E):
+  Hint Constructors ktrans_: ctl.
+  
+  Local Instance ktrans_equ_aux1 {X}(t: ctree' E X) (w: World E):
     Proper (going (equ eq) ==> eq ==> flip impl) (ktrans_ t w).
   Proof.
     unfold Proper, respectful, iff, fst, snd; cbn; unfold fst, snd;
@@ -65,7 +67,7 @@ Section CTreeTrans.
       rename u into U;
       remember ({| _observe := U |}) as u;
       replace U with (observe u) in * by now subst.
-    - eapply KtransTau; auto.
+    - eapply KtransGuard; auto.
     - eapply KtransBr; auto.
       transitivity t; eauto.
       now step.
@@ -80,7 +82,7 @@ Section CTreeTrans.
       now step.
   Qed.
 
-  Global Instance ktrans_equ_aux2:
+  Global Instance ktrans_equ_aux2{X}:
     Proper (going (equ eq) ==> eq ==> going (equ eq) ==> eq ==> impl) (ktrans_ (X:=X)).
   Proof.
     intros t t' Heqt x x' <- u u' Hequ y y' <- TR.
@@ -89,7 +91,7 @@ Section CTreeTrans.
     revert t' eqt.
     dependent induction TR; intros; auto.
     + step in eqt; cbn in eqt; dependent destruction eqt.
-      eapply KtransTau; eauto.
+      eapply KtransGuard; eauto.
       eapply IHTR; auto.
       now rewrite <- !ctree_eta.
     + step in eqt; cbn in eqt; dependent destruction eqt.
@@ -114,9 +116,10 @@ Section CTreeTrans.
   Next Obligation.
     dependent induction H; cbn; eauto with ctl; inv H0.
   Defined.
+  Hint Unfold ktrans: ctl.
   Arguments ktrans /.
   
-  Global Instance ktrans_equ_proper:
+  Global Instance ktrans_equ_proper{X}:
     Proper (equ eq ==> eq ==> equ eq ==> eq ==> iff) (ktrans (X:=X)).
   Proof.
     unfold Proper, respectful, RelCompFun, fst, snd; cbn; intros; subst.
@@ -125,24 +128,88 @@ Section CTreeTrans.
     - now rewrite H, H1.
   Qed.
 
-  Global Instance KripkeSetoidEqu: @KripkeSetoid (ctree E) E HE ctree_kripke X (equ eq) _.
-  Proof.
-    repeat red.
-    intros.
-    setoid_rewrite <- H.
-    exists s'; auto.
-  Defined.
-End CTreeTrans.
+  (*| Prove [trans], [ktrans] are in lockstep and worlds/labels are 1-1 |*)
+  Lemma ktrans_trans{X}: forall (t t': ctree E X) w w',
+      ktrans_ (observe t) w (observe t') w' <->
+        (exists l, trans_ l (observe t) (observe t') /\
+                ((l = tau /\ not_done w /\ w' = w)
+                 \/ (exists e (x: encode e), l = obs e x /\ not_done w /\ w' = Obs e x)
+                 \/ (exists (x: X), l = val x /\ w = Pure /\ t' ≅ stuck /\ w' = Done x)
+                 \/ (exists e (v: encode e) (x: X), l = val x /\ w = Obs e v /\ t' ≅ stuck /\ w' = Finish e v x))).
+  Proof with eauto with ctree.
+    intros; split; intro H.
+    - remember (observe t) as T; remember (observe t') as T';
+      generalize dependent t; generalize dependent t'.
+      induction H; intros; subst.
+      + destruct (IHktrans_ _ HeqT' _ eq_refl) as (l & TR & Hl). 
+        exists l; split...
+        apply trans_guard...
+      + exists tau; split... 
+        apply trans_br with (x:=i).
+        now symmetry. 
+      + exists (obs e v); split.
+        * econstructor; now symmetry.
+        * right; left.
+          exists e, v...
+      + exists (val x); rewrite H; split.
+        * now econstructor.
+        * right; right; left.
+          exists x; intuition.
+          transitivity t...
+          step; cbn; rewrite HeqT'; reflexivity.
+      + exists (val x); rewrite H; split; auto.
+        * now econstructor.
+        * right; right; right.
+          exists e, v, x; intuition.
+          transitivity t...
+          step; cbn; rewrite HeqT'; reflexivity.
+    - destruct H as (l & ? & Hl);
+      remember (observe t) as T; remember (observe t') as T';
+        generalize dependent t; generalize dependent t'; revert w w'.
+      induction H; intros; subst.
+      + apply KtransGuard...
+      + destruct Hl as [ (? & ? & ?) |
+             [(e & x' & ? & ? & ?) |
+               [(x' & ? & ? & Ht & ?) |
+                 (e & v & x' & ? & ? & Ht & ?)]]];
+          subst; inv H0.
+        apply KtransBr with x... 
+        now symmetry.
+      + destruct Hl as [ (? & ? & ?) |
+             [(e' & x' & ? & ? & ?) |
+               [(x' & ? & ? & Ht & ?) |
+                 (e' & v & x' & ? & ? & Ht & ?)]]]; subst;
+          dependent destruction H0.
+        apply KtransObs; auto.
+        now symmetry.
+      + destruct Hl as [ (? & ? & ?) |
+             [(e' & x' & ? & ? & ?) |
+               [(x' & ? & ? & Ht & ?) |
+                 (e' & v & x' & ? & ? & Ht & ?)]]]; subst;
+          dependent destruction H0.
+        * apply KtransDone.
+          transitivity t'; auto.
+          step; cbn; rewrite HeqT'; reflexivity.
+        * apply KtransFinish.
+          transitivity t'; auto.
+          step; cbn; rewrite HeqT'; reflexivity.
+  Qed.
 
-Global Hint Constructors ktrans_: core.
+  (* Here I define two setoid instaces, one for [equ eq]
+     and one for [sbisim eq]. Even though [equ eq] is a subrelation
+     of [sbisim eq], I had to delete the subrelation instance and
+     duplicate here because instance resolution became extremely slow. *)
+  Global Instance KripkeSetoidEqu {X}:
+    @KripkeSetoid (ctree E) E HE ctree_kripke X (equ eq) _.
+  Proof.    
+    repeat red; intros.
+    rewrite H in H0.
+    exists s'; intuition.
+  Qed.
 
-(*| Lemmas that depend on structure of [ctrees] |*)
-Section CTreeTransLemmas.
-  Context {E: Type} `{HE: Encode E}.
-  Local Open Scope ctl_scope.  
-
-  Lemma ktrans_tau {X}: forall (t t': ctree E X) w w',
-      [Tau t, w] ↦ [t', w'] <-> [t, w] ↦ [t', w'].
+  Local Open Scope ctl_scope.
+  Lemma ktrans_guard{X}: forall (t t': ctree E X) w w',
+      [Guard t, w] ↦ [t', w'] <-> [t, w] ↦ [t', w'].
   Proof.
     split; intro H.
     - cbn in H; dependent induction H; cbn in *.
@@ -150,7 +217,8 @@ Section CTreeTransLemmas.
     - cbn in *.
       now econstructor.
   Qed.
-
+  Hint Resolve ktrans_guard: ctl.
+  
   Lemma ktrans_br {X}: forall n (t: ctree E X) (k: fin' n -> ctree E X) w w',
       [Br n k, w] ↦ [t, w'] <->
         (exists (i: fin' n), t ≅ k i /\ w = w' /\ not_done w).
@@ -163,6 +231,7 @@ Section CTreeTransLemmas.
     - destruct H as (i & Heq & -> & Hd).
       econstructor; eauto.
   Qed.
+  Hint Resolve ktrans_br: ctl.
   
   Lemma ktrans_done {X}: forall (t: ctree E X) (w': World E) x,
       [Ret x, Pure] ↦ [t, w'] <-> (w' = Done x /\ t ≅ stuck).
@@ -173,7 +242,8 @@ Section CTreeTransLemmas.
     - destruct H as (-> & ->); constructor.
       reflexivity. 
   Qed.
-
+  Hint Resolve ktrans_done: ctl.
+  
   Lemma ktrans_finish {X}: forall (t: ctree E X) (w': World E) (e: E) (v: encode e) x,
       [Ret x, Obs e v] ↦ [t, w'] <->
         (w' = Finish e v x /\ t ≅ stuck).
@@ -184,7 +254,8 @@ Section CTreeTransLemmas.
     - destruct H as (-> & ->); constructor.
       reflexivity. 
   Qed.
-
+  Hint Resolve ktrans_finish: ctl.
+  
   Lemma ktrans_vis{X}: forall (t: ctree E X) (s s': World E) (e: E) (k: encode e -> ctree E X),
       [Vis e k, s] ↦ [t, s'] <->
         (exists (x: encode e), s' = Obs e x /\ k x ≅ t /\ not_done s).
@@ -198,7 +269,8 @@ Section CTreeTransLemmas.
     - destruct TR as (? & -> & <- & ?).
       econstructor; auto.
   Qed.
-
+  Hint Resolve ktrans_vis: ctl.
+  
   Lemma ktrans_pure_pred{X}: forall (t t': ctree E X) w,
       [t, w] ↦ [t', Pure] -> w = Pure.
   Proof.
@@ -223,19 +295,50 @@ Section CTreeTransLemmas.
     inv Hret;
       apply ktrans_not_done in H; inv H.
   Qed.
-
+  Hint Resolve done_not_ktrans: ctl.
+  
   Lemma ktrans_done_inv{X}: forall (t t': ctree E X) (x: X) w,
       ~ [t, Done x] ↦ [t', w].
   Proof.
     intros * Hcontra; cbn in Hcontra; dependent induction Hcontra; eauto; inv H.
   Qed.
+  Hint Resolve ktrans_done_inv: ctl.
   
   Lemma ktrans_finish_inv{X}: forall (t t': ctree E X) (e: E) (v: encode e) (x: X) w,
       ~ [t, Finish e v x] ↦ [t', w].
   Proof.
     intros * Hcontra; cbn in Hcontra; dependent induction Hcontra; eauto; inv H.
   Qed.
-
+  Hint Resolve ktrans_finish_inv: ctl.
+  
+  Lemma ktrans_to_done_inv{X}: forall (t t': ctree E X) w (x: X),
+      [t, w] ↦ [t', Done x] ->
+      t' ≅ Ctree.stuck /\ w = Pure.
+  Proof.
+    intros.
+    cbn in H.
+    dependent induction H; intros; eauto.
+    - inv H.
+    - observe_equ x.
+      rewrite Eqt in H.
+      intuition.
+  Qed.
+  Hint Resolve ktrans_to_done_inv: ctl.
+  
+  Lemma ktrans_to_finish_inv{X}: forall (t t': ctree E X) w (e: E) (v: encode e) (x: X),
+      [t, w] ↦ [t', Finish e v x] ->
+      t' ≅ Ctree.stuck /\ w = Obs e v.
+  Proof.
+    intros.
+    cbn in H.
+    dependent induction H; intros; eauto.
+    - inv H.
+    - observe_equ x.
+      rewrite Eqt in H.
+      intuition.
+  Qed.
+  Hint Resolve ktrans_to_finish_inv: ctl.
+  
   Lemma ktrans_bind_l{X Y}: forall (t t': ctree E Y) (k: Y -> ctree E X) w w',
       [t, w] ↦ [t', w'] ->
       not_done w' ->
@@ -273,24 +376,25 @@ Section CTreeTransLemmas.
     intros.
     generalize dependent y.
     cbn in H; dependent induction H; intros.
-    - assert(Hx: t ≅ Tau t0) by (step; cbn; rewrite <- x0; reflexivity).
-      setoid_rewrite Hx.
-      rewrite bind_tau.
+    - assert(Hx: t ≅ Guard t0) by (step; cbn; rewrite <- x0; reflexivity).
+      rewrite Hx.
+      rewrite bind_guard.
       econstructor.
       eapply IHktrans_; eauto.
     - inv H1; inv H.
     - inv H1.
     - dependent destruction H0.
       observe_equ x1.
-      setoid_rewrite Eqt.
+      rewrite Eqt.
       now rewrite bind_ret_l.
     - dependent destruction H0.
       observe_equ x1.
       setoid_rewrite Eqt.
       now rewrite bind_ret_l.
   Qed.      
-
-  Opaque Ctree.stuck.
+  Typeclasses Opaque equ.
+  
+  Opaque Ctree.stuck.  
   Lemma ktrans_bind_inv_aux {X Y} (w w': World E)(T U: ctree' E Y) :
     ktrans_ T w U w' ->
     forall (t: ctree E X) (k: X -> ctree E Y) (u: ctree E Y),
@@ -300,16 +404,10 @@ Section CTreeTransLemmas.
       (exists t', [t, w] ↦ [t', w']        
              /\ not_done w'
              /\ u ≅ x <- t' ;; k x) \/
-        (* [t] pure return [Done x], [t>>=k] steps if [k x] steps *)
-      (exists (x: X),                      
-          [t, w] ↦ [stuck, Done x]
-          /\ w = Pure
-          /\ [k x, Pure] ↦ [u, w']) \/
-        (* [t] impure return [Finish e v x], [t>>=k] steps if [k x] steps *)
-      (exists (e: E) (v: encode e) (x: X), 
-          [t, w] ↦ [stuck, Finish e v x]
-          /\ w = Obs e v
-          /\ [k x, Obs e v] ↦ [u, w']).
+        (* [t] returns [x], [t>>=k] steps if [k x] steps *)
+        (exists y w_, [t, w] ↦ [stuck, w_]
+                 /\ done_eq X y w_
+                 /\ [k y, w] ↦ [u, w']).
   Proof with (auto with ctl).
     intros TR.
     dependent induction TR; intros.
@@ -317,37 +415,34 @@ Section CTreeTransLemmas.
         desobs t0; observe_equ Heqt.
       + right.
         pose proof (ktrans_not_done (X:=Y) t t' w w' TR) as Hw.
-        inv Hw.
-        * left; exists x.
+        inv Hw; exists x.        
+        * exists (Done x). 
           split; [|split]...
-          rewrite <- H, <- H0; cbn; now apply KtransTau.
-        * right; exists e, v, x.
+          rewrite <- H, <- H0; cbn; now apply KtransGuard.
+        * exists (Finish e v x). 
           split; [|split]... 
-          rewrite <- H, <- H0; cbn; now apply KtransTau.
+          rewrite <- H, <- H0; cbn; now apply KtransGuard.
       + step in H; inv H.
-      + pose proof (equ_tau_invE H).
+      + pose proof (equ_guard_invE H).
         rewrite ctree_eta in H1.
         destruct (IHTR _ _ _ H1 H0)
           as [(t2 & TR2 & Hd & Eq2) |
-               [(x & TRr & -> & TRk) |
-                 (e & v & x & TRr & -> & TRk)]].
+               (x & w_ & TRr & ? & TRk)].
         * left.
           exists t2; split; [|split]... 
-        * right; left.
-          exists x.
-          split... 
-        * right; right.
-          exists e, v, x.
-          split...
+        * right.
+          inv H2.
+          -- exists x0, (Done x0); split...
+          -- exists x0, (Finish e v x0); split...
       + step in H; inv H.
     - rewrite unfold_bind in H1; unfold ktrans; cbn; desobs t0; observe_equ Heqt.
       + right; inv H.
-        * left; exists x.
+        * exists x, (Done x).
           split; [|split]... 
           rewrite <- H1; cbn; apply KtransBr with i... 
           rewrite <- ctree_eta in H2.
           transitivity t; [symmetry|]... 
-        * right; exists e, v, x. 
+        * exists x, (Finish e v x). 
           split; [|split]... 
           rewrite <- H1; cbn; apply KtransBr with i... 
           rewrite <- ctree_eta in H2.
@@ -363,12 +458,12 @@ Section CTreeTransLemmas.
       + step in H1; inv H1.
     - rewrite unfold_bind in H1; unfold ktrans; cbn; desobs t0; observe_equ Heqt.
       + right; inv H.
-        * left; exists x.
+        * exists x, (Done x).
           split; [|split]... 
           rewrite <- H1; cbn; apply KtransObs... 
           rewrite <- ctree_eta in H2.
           transitivity t; [symmetry|]... 
-        * right; exists e0, v0, x. 
+        * exists x, (Finish e0 v0 x). 
           split; [|split]... 
           rewrite <- H1; cbn; apply KtransObs... 
           rewrite <- ctree_eta in H2.
@@ -383,8 +478,8 @@ Section CTreeTransLemmas.
         now rewrite <- ctree_eta.       
     - rewrite unfold_bind in H0; unfold ktrans; cbn;
         desobs t0; observe_equ Heqt.
-      + right; left.
-        exists x0.
+      + right. 
+        exists x0, (Done x0).
         split; [|split]...
         rewrite <- H1, H, <- H0; cbn.
         now apply KtransDone.
@@ -393,8 +488,8 @@ Section CTreeTransLemmas.
       + step in H0; inv H0.
     - rewrite unfold_bind in H0; unfold ktrans; cbn;
         desobs t0; observe_equ Heqt.
-      + right; right.
-        exists e, v, x0.
+      + right. 
+        exists x0, (Finish e v x0).
         split; [|split]...
         rewrite <- H1, H, <- H0; cbn.
         now apply KtransFinish.
@@ -403,20 +498,16 @@ Section CTreeTransLemmas.
       + step in H0; inv H0.
   Qed.
 
-   Lemma ktrans_bind_inv: forall {X Y} (w w': World E)
+  Lemma ktrans_bind_inv: forall {X Y} (w w': World E)
                            (t: ctree E X) (u: ctree E Y) (k: X -> ctree E Y),
       [x <- t ;; k x, w] ↦ [u, w'] ->
       (exists t', [t, w] ↦ [t', w']
              /\ not_done w'
              /\ u ≅ x <- t' ;; k x) \/
-      (exists (x: X),              
-          [t, w] ↦ [stuck, Done x]
-          /\ w = Pure
-          /\ [k x, Pure] ↦ [u, w']) \/
-      (exists (e: E) (v: encode e) (x: X),
-          [t, w] ↦ [stuck, Finish e v x]
-          /\ w = Obs e v
-          /\ [k x, Obs e v] ↦ [u, w']).
+        (* [t] returns [x], [t>>=k] steps if [k x] steps *)
+        (exists y w_, [t, w] ↦ [stuck, w_]
+                 /\ done_eq X y w_
+                 /\ [k y, w] ↦ [u, w']).
   Proof.
     intros * TR.
     eapply ktrans_bind_inv_aux.
@@ -424,8 +515,9 @@ Section CTreeTransLemmas.
     rewrite <- ctree_eta; reflexivity.
     rewrite <- ctree_eta; reflexivity.
   Qed.
+  Hint Resolve ktrans_bind_inv: ctl.
   
-End CTreeTransLemmas.
+End CTreeTrans.
 
 Local Typeclasses Transparent equ.
 Local Open Scope ctl_scope.
@@ -436,13 +528,54 @@ Proof.
   intros.
   unfold trigger in H3.
   apply ktrans_bind_inv in H3 as
-      [(t' & TR & Hd & Hequ) | [(x & TR & ? & ?) | (e' & v' & x' & TR & -> & TR')]].
+      [(t' & TR & Hd & Hequ) |
+        (x & w_ & TRr & ? & TRk)].
   - apply ktrans_vis in TR as (y & ? & ? & ?).
     unfold resum, ReSum_refl, resum_ret, ReSumRet_refl in *; world_inv.
     split; [auto | exists y]; split; [reflexivity|].
     now rewrite <- H4, bind_ret_l in Hequ.
-  - apply ktrans_vis in TR as (y & ? & ? & ?); subst.
-    step in H6; cbn in H6; inv H6.
-  - apply ktrans_vis in TR as (y & ? & ? & ?); subst.
-    step in H4; cbn in H4; inv H4.
+  - apply ktrans_vis in TRr as (y & ? & ? & ?); subst.
+    inv H3.
 Qed.
+
+Global Hint Constructors
+  ktrans_ not_done done_with vis_with: ctl.
+
+Global Hint Resolve
+  ktrans_stuck ktrans_br ktrans_vis ktrans_done
+  ktrans_done_inv ktrans_finish can_step_not_done
+  ktrans_not_done ktrans_finish_inv ktrans_bind_inv
+  ktrans_to_done_inv ktrans_to_finish_inv
+  ktrans_guard ktrans_pure_pred: ctl.
+
+From CTree Require Import CTree.SBisim.
+Local Typeclasses Opaque equ.      
+Global Instance KripkeSetoidSBisim{E} {HE: Encode E} {X}:
+    @KripkeSetoid (ctree E) E HE ctree_kripke X (sbisim eq) _.
+Proof.    
+  repeat red; intros.
+  apply ktrans_trans in H0 as
+      (l & TR &
+         [ (? & ? & ?) |
+           [(e & x & ? & ? & ?) |
+             [(x & ? & ? & Ht & ?) |
+               (e & v & x & ? & ? & Ht & ?)]]]); subst;
+    destruct (SBisim.sbisim_trans (X:=X) _ _ _ _ eq H TR)
+    as (l' & c1' & ? & <- & ?); exists c1'.
+  - split; [apply ktrans_trans|auto].
+    exists tau; split; auto. 
+  - split; [apply ktrans_trans|auto].
+    exists (obs e x); split; auto.
+    right; left.
+    exists e, x; intuition.
+  - split; [apply ktrans_trans|auto].
+    exists (val x); split; auto.
+    right; right; left.
+    pose proof trans_val_inv H0.
+    exists x; intuition. 
+  - split; [apply ktrans_trans|auto].
+    exists (val x); split; auto.
+    right; right; right.
+    pose proof trans_val_inv H0.
+    exists e, v, x; intuition.
+Defined.
