theories/CTree/Logic/AX.v
@@ -10,6 +10,7 @@ From CTree Require Import
   Events.Core
   CTree.Core
   CTree.Equ
+  CTree.SBisim
   CTree.Logic.Trans
   CTree.Logic.CanStep
   Logic.Ctl
@@ -37,19 +38,22 @@ Section BasicLemmas.
     inv Hret; inv H.
   Qed.
 
-  Lemma ax_tau: forall (t: ctree E X) w φ,
-      <( {Tau t}, w |= AX now φ )> <->
-      <( t, w |= AX now φ )>.
-  Proof with auto with ctl.
-    split; intros; destruct H as [(t' & w' & TR) H].   
-    - split.
-      * rewrite ktrans_tau in TR...
-      * intros t_ w_ TR_.
-        apply ktrans_tau in TR_...
-    - split.
-      * apply can_step_tau...
-      * intros t_ w_ TR_.
-        rewrite ktrans_tau in TR_...
+  Lemma ax_stuck: forall w φ,
+      <( {Ctree.stuck: ctree E X}, w |= AX φ )> ->
+      <( {Ctree.stuck: ctree E X}, w |= φ )>.
+  Proof.
+    intros.
+    cbn in H; dependent induction H; auto.
+    apply can_step_stuck in H.
+    contradiction.
+  Qed.
+
+  Lemma ax_guard: forall (t: ctree E X) w φ,
+      <( {Guard t}, w |= AX φ )> <->
+      <( t, w |= AX φ )>.
+  Proof.
+    intros.
+    now rewrite sb_guard.
   Qed.
   
   Lemma ax_br: forall n (k: fin' n -> ctree E X) w φ,
@@ -90,35 +94,115 @@ Section BasicLemmas.
         apply H0.
   Qed.
 
-  Lemma ax_done: forall (x: X) φ,
-      <( {Ret x}, Pure |= AX done φ )> <-> φ x Pure. 
-  Proof with auto with ctl.
+  Lemma ax_done: forall (x: X) φ w,
+      <( {Ret x}, w |= AX done φ )> <-> not_done w /\ φ x w. 
+  Proof.
     split; intros.
     - next in H; destruct H.
       destruct H as (t' & w' & TR).
       specialize (H0 _ _ TR).
-      apply ktrans_done in TR as (-> & ?).
-      inv H0; now invert. 
-    - split.
-      + apply can_step_ret...
+      split.
+      + now apply ktrans_not_done with (Ret x) t' w'.
+      + cbn in TR.
+        dependent destruction TR; observe_equ x;
+          rewrite <- Eqt in H0;
+          now apply ctl_done in H0;
+          dependent destruction H0.
+    - split; destruct H.
+      + now apply can_step_ret.
       + intros t' w' TR.
-        apply ktrans_done in TR as (-> & ->).
-        now constructor.
+        inv H.
+        * apply ktrans_done in TR as (? & ->).
+          apply ctl_done; subst.
+          now constructor.
+        * apply ktrans_finish in TR as (-> & ->).
+          apply ctl_done.
+          now constructor.
   Qed.
 
-  Lemma ax_finish: forall (x: X) (e: E) (v: encode e) φ,
-      <( {Ret x}, {Obs e v} |= AX done φ )> <-> φ x (Obs e v). 
-  Proof with auto with ctl.
-    split; intros.
-    - next in H; destruct H.
-      destruct H as (t' & w' & TR).
-      specialize (H0 _ _ TR).
-      apply ktrans_finish in TR as (-> & ?).
-      inv H0; now invert. 
-    - split.
-      + apply can_step_ret...
-      + intros t' w' TR.
-        apply ktrans_finish in TR as (-> & ->).
-        now constructor.
-  Qed.
 End BasicLemmas.
+
+Section BindLemmas.
+  Context {E: Type} {HE: Encode E}.
+
+  Theorem ax_bind_vis{X Y}: forall (t: ctree E Y) (k: Y -> ctree E X) φ w,
+      <( t, w |= AX vis φ )> ->
+      <( {x <- t ;; k x}, w |= AX vis φ )>.
+  Proof with auto with ctl.
+    intros.
+    next in H.
+    destruct H as [(t' & w' & TR') Hs].
+    next; split.
+    + specialize (Hs _ _ TR').
+      apply ctl_vis in Hs; inv Hs.
+      eapply can_step_bind_l with t' (Obs e v)...
+    + intros t_ w_ TR_.
+      clear t' w' TR' w'.
+      apply ktrans_bind_inv in TR_ as
+          [(t' & TR' & Hd & Ht_) |
+            (x & w' & TR' & Hr & TRk)].
+      * now eapply (Hs t').
+      * dependent destruction Hr;
+        specialize (Hs _ _ TR');
+        apply ctl_vis in Hs; inv Hs. 
+  Qed.
+
+  Theorem ax_bind_pure{X Y}: forall (t: ctree E Y) (k: Y -> ctree E X) w,
+      <( t, w |= AX pure )> ->
+      <( {x <- t ;; k x}, w |= AX pure )>.
+  Proof with auto with ctl.
+    intros.
+    next in H.
+    destruct H as [(t' & w' & TR') Hs].
+    next; split.
+    + specialize (Hs _ _ TR').
+      apply ctl_pure in Hs as ->.
+      eapply can_step_bind_l with t' Pure... 
+    + intros t_ w_ TR_.
+      clear t' w' TR' w'.
+      apply ktrans_bind_inv in TR_ as
+          [(t' & TR' & Hd & Ht_) |
+            (x & w' & TR' & Hr & TRk)].
+      * now eapply (Hs t').
+      * dependent destruction Hr;
+        specialize (Hs _ _ TR');
+        apply ctl_pure in Hs; inv Hs. 
+  Qed.
+
+  Opaque Ctree.stuck.
+  Theorem ax_bind_r{X Y}: forall (t: ctree E Y) (k: Y -> ctree E X) w φ R,
+      <( t, w |= AX done R )> ->
+      (forall x w, R x w -> <( {k x}, w |= AX φ )>) ->
+      <( {x <- t ;; k x}, w |= AX φ )>.
+  Proof.
+    intros.
+    next; split.
+    - apply can_step_bind_r with R.
+      + now next; left.
+      + intros y w' HR.
+        specialize (H0 y w' HR).
+        now next in H0; destruct H0.
+    - intros t' w' TR'. 
+      apply ktrans_bind_inv in TR' as
+          [(t_ & TR_ & Hd & ->) |
+            (x & w_ & TR_ & Hr & TRk)].
+      + next in H; destruct H.
+        specialize (H1 _ _ TR_).
+        apply ctl_done in H1; inv H1; inv Hd.
+      + next in H; destruct H.
+        specialize (H1 _ _ TR_).
+        apply ctl_done in H1.       
+        dependent destruction H1; dependent destruction Hr.
+        * specialize (H1 _ _ H0).
+          next in H1.
+          destruct H1 as (Hs & Ht').
+          apply Ht'.
+          now apply ktrans_to_done_inv in TR_ as (_ & ->). 
+        * specialize (H1 _ _ H0).
+          next in H1.
+          destruct H1 as (Hs & Ht').
+          apply Ht'.
+          now apply ktrans_to_finish_inv in TR_ as (_ & ->). 
+  Qed.
+End BindLemmas.
+
