theories/CTree/SBisim/Core.v
@@ -1,0 +1,1354 @@
+From Coq Require Import
+     Lia
+     Basics
+     Fin
+     RelationClasses
+     Program.Equality
+     Logic.Eqdep.
+
+From Coinduction Require Import
+     coinduction rel tactics.
+
+From CTree Require Import
+  CTree.Core
+  CTree.Equ
+  CTree.Trans
+  CTree.SBisim.SSim.
+
+Local Open Scope ctree_scope.
+Set Implicit Arguments.
+Generalizable All Variables.
+
+Arguments pointwise_relation /.
+Arguments Proper /.
+Arguments respectful /.
+Arguments impl /.
+Arguments flip /.
+
+Section StrongBisim.
+  Context {E F: Type} {HE: Encode E} {HF: Encode F} {X Y : Type}.
+  Notation S := (ctree E X).
+  Notation S' := (ctree F Y).
+
+  (*| The symmetric closure of two [ss] |*)
+  Program Definition sb L : mon (S -> S' -> Prop) :=
+    {| body R t u := ss L R t u /\ ss (flip L) (flip R) u t |}.
+  Next Obligation.
+    split; intros.
+    - destruct (H0 _ _ H2) as (? & ? & ? & ? & ?).
+      exists x0, x1; auto.
+    - destruct (H1 _ _ H2) as (? & ? & ? & ? & ?); unfold flip in *.
+      exists x0, x1; auto.      
+  Qed.
+
+  #[global] Instance weq_sb : Proper (weq ==> weq) sb.
+  Proof.
+    split; intros.
+    - split.
+      + epose proof (weq_ss H). cbn in H1. setoid_rewrite <- H1. apply H0.
+      + cbn in H. assert (flip x == flip y).
+        { cbn. split; intro. apply H. apply H1. apply H. apply H1. }
+        epose proof (weq_ss H1).
+        cbn in H2. setoid_rewrite <- H2. apply H0.
+    - split.
+      + epose proof (weq_ss H). cbn in H1. setoid_rewrite H1. apply H0.
+      + cbn in H. assert (flip x == flip y).
+        { cbn. split; intro. apply H. apply H1. apply H. apply H1. }
+        epose proof (weq_ss H1).
+        cbn in H2. setoid_rewrite H2. apply H0.
+  Qed.
+
+  Definition sbisim L := gfp (sb L).
+
+  #[global] Instance weq_sbisim : 
+      Proper (weq ==> weq) sbisim.
+  Proof.
+    intros. split.
+    - intro. unfold sbisim.
+      epose proof (gfp_weq (sb x) (sb y)). lapply H1.
+      + intro. red in H2. cbn in H2. rewrite <- H2. unfold sbisim in H0. apply H0.
+      + now rewrite H.
+    - intro. unfold sbisim.
+      epose proof (gfp_weq (sb x) (sb y)). lapply H1.
+      + intro. red in H2. cbn in H2. rewrite H2. unfold sbisim in H0. apply H0.
+      + now rewrite H.
+  Qed.
+
+End StrongBisim.
+
+(* This instance allows to use the symmetric tactic from coq-coinduction
+   for homogeneous bisimulations *)
+#[global] Instance sbisim_sym `{HE: Encode E} {X} {L: rel (label E) (label E) }
+  {HL: Symmetric L}:
+    Sym_from converse (sb (X:=X) L) (ss L).
+  Proof.
+    split; intro.
+    - destruct H. split.
+      + apply H.
+      + cbn. intros. apply H0 in H1 as (? & ? & ? & ? & ?). apply HL in H3. eauto.
+    - destruct H. split.
+      + apply H.
+      + cbn. intros. apply H0 in H1 as (? & ? & ? & ? & ?). apply HL in H3. eauto.
+  Qed.
+
+Local Open Scope ctree_scope.
+
+(*| sb (bisimulation) notation |*)
+Local Notation st L := (t (sb L)).
+Local Notation sT L := (T (sb L)).
+Local Notation sbt L := (bt (sb L)).
+Local Notation sbT L := (bT (sb L)).
+
+Notation "t ~ u" := (sbisim eq t u) (at level 70): ctree_scope.
+Notation "t (~ L ) u" := (sbisim L t u) (at level 70): ctree_scope.
+Notation "t [~ L] u" := (st L _ t u) (at level 78): ctree_scope.
+Notation "t [~] u" := (st eq _ t u) (at level 78): ctree_scope.
+Notation "t {~ L } u" := (sbt L _ t u) (at level 79): ctree_scope.
+Notation "t {~} u" := (sbt eq _ t u) (at level 79): ctree_scope.
+Notation "t {{ ~ L }} u" := (sb L _ t u) (at level 79): ctree_scope.
+Notation "t {{~}} u" := (sb eq _ t u) (at level 79): ctree_scope.
+
+Ltac fold_sbisim :=
+  repeat
+    match goal with
+    | h: context[gfp (@sb ?E ?F ?C ?D ?X ?Y ?L)] |- _  => fold (@sbisim E F C D X Y L) in h
+    | |- context[gfp (@sb ?E ?F ?C ?D ?X ?Y ?L)]       => fold (@sbisim E F C D X Y L)
+    end.
+
+Ltac __coinduction_sbisim R H :=
+  (try unfold sbisim);
+  apply_coinduction; fold_sbisim; intros R H.
+
+#[global] Tactic Notation "__step_sbisim" :=
+  match goal with
+  | |- context[@sbisim ?E ?F ?C ?D ?X ?Y ?LR] =>
+      unfold sbisim;
+      step;
+      fold (@sbisim E F C D X Y L)
+  end.
+
+#[local] Tactic Notation "step" := __step_sbisim || __step_ssim || step.
+
+#[local] Tactic Notation "coinduction" simple_intropattern(R) simple_intropattern(H) :=
+  __coinduction_sbisim R H || __coinduction_ssim R H || coinduction R H.
+
+Ltac __step_in_sbisim H :=
+  match type of H with
+  | context [@sbisim ?E ?F ?C ?D ?X ?Y ?L ] =>
+      unfold sbisim in H;
+      step in H;
+      fold (@sbisim E F C D X Y L) in H
+  end.
+
+#[local] Tactic Notation "step" "in" ident(H) := __step_in_sbisim H || __step_in_ssim H || step in H.
+
+(*|
+  This section should describe lemmas proved for the
+  heterogenous version of `ss`, parametric on
+  - Return types X, Y
+  - Label types E, F
+|*)
+Section sbisim_heterogenous_theory.
+  Context `{HE: Encode E} `{HF: Encode F} {X Y : Type}
+          {L: rel (label E) (label F)}.
+
+  Local Notation sb := (@sb E F HE HF X Y).
+  Local Notation sbisim := (@sbisim E F HE HF X Y).
+  Local Notation st L := (coinduction.t (sb L)).
+  Local Notation sbt L := (coinduction.bt (sb L)).
+  Local Notation sT  L := (coinduction.T (sb L)).
+
+  (*| Strong bisimulation up-to [equ] is valid |*)
+  Lemma equ_clos_st : @equ_clos E F X Y HE HF <= (st L).
+  Proof.
+    apply Coinduction; cbn.
+    intros R x y [x' y' x'' y'' EQ' [Fwd Back] EQ'']; split.
+    - intros l z x'z.
+      rewrite EQ' in x'z.
+      apply Fwd in x'z.
+      destruct x'z as (? & ? & ? & ? & ?).
+      do 2 eexists; intuition.
+      rewrite <- EQ''; eauto.
+      eapply (f_Tf (sb L)).
+      econstructor; eauto.
+      assumption.
+    - intros l z y'z.
+      rewrite <- EQ'' in y'z.
+      apply Back in y'z.
+      destruct y'z as (? & ? & ? & ? & ?).
+      do 2 eexists; intuition.
+      rewrite EQ'; eauto.
+      eapply (f_Tf (sb L)).
+      econstructor; eauto.
+      eauto.
+  Qed.
+
+(*|
+    Aggressively providing instances for rewriting [equ] under all [sb]-related
+    contexts.
+|*)
+  #[global] Instance equ_clos_st_goal RR :
+    Proper (@equ E HE X X eq ==> @equ F HF Y Y eq ==> flip impl) (st L RR).
+  Proof.
+    cbn; intros ? ? eq1 ? ? eq2 H.
+    apply (ft_t equ_clos_st); econstructor; [eauto | | symmetry; eauto]; assumption.
+  Qed.
+
+  #[global] Instance equ_clos_st_ctx RR :
+    Proper (@equ E HE X X eq ==> @equ F HF Y Y eq ==> impl) (st L RR).
+  Proof.
+    cbn; intros ? ? eq1 ? ? eq2 H.
+    apply (ft_t equ_clos_st); econstructor; [symmetry; eauto | | eauto]; assumption.
+  Qed.
+
+  #[global] Instance equ_clos_sT_goal RR f :
+    Proper (equ eq ==> equ eq ==> flip impl) (sT L f RR).
+  Proof.
+    cbn; intros ? ? eq1 ? ? eq2 H.
+    apply (fT_T equ_clos_st); econstructor; [eauto | | symmetry; eauto]; assumption.
+  Qed.
+
+  #[global] Instance equ_clos_sT_ctx RR f :
+    Proper (equ eq ==> equ eq ==> impl) (sT L f RR).
+  Proof.
+    cbn; intros ? ? eq1 ? ? eq2 H.
+    apply (fT_T equ_clos_st); econstructor; [symmetry; eauto | | eauto]; assumption.
+  Qed.
+
+  #[global] Instance equ_clos_sbisim_goal :
+    Proper (equ eq ==> equ eq ==> flip impl) (sbisim L).
+  Proof.
+    cbn; intros ? ? eq1 ? ? eq2 H.
+    apply (ft_t equ_clos_st); econstructor; [eauto | | symmetry; eauto]; assumption.
+  Qed.
+
+  #[global] Instance equ_clos_sbisim_ctx :
+    Proper (equ eq ==> equ eq ==> impl) (sbisim L).
+  Proof.
+    cbn; intros ? ? eq1 ? ? eq2 H.
+    apply (ft_t equ_clos_st); econstructor; [symmetry; eauto | | eauto]; assumption.
+  Qed.
+
+  #[global] Instance equ_ss_closed_goal {r} : Proper (@equ E HE X X eq ==> @equ F HF Y Y eq ==> flip impl) (ss L r).
+  Proof.
+    intros t t' tt' u u' uu'; cbn; intros.
+    rewrite tt' in H0. apply H in H0 as (? & ? & ? & ? & ?).
+    eexists; eexists; eauto. rewrite uu'. eauto.
+  Qed.
+
+  #[global] Instance equ_ss_closed_ctx {r} : Proper (@equ E HE X X eq ==> @equ F HF Y Y eq ==> impl) (ss L r).
+  Proof.
+    intros t t' tt' u u' uu'; intros.
+    rewrite tt', uu'. reflexivity.
+  Qed.
+
+  (*| Up-to-bisimulation enhancing function |*)
+  Variant sbisim_clos_body {LE LF}
+          (R : rel (ctree E X) (ctree F Y)) : (rel (ctree E X) (ctree F Y)) :=
+    | Sbisim_clos : forall t t' u' u
+                      (Sbisimt : t (~ LE) t')
+                      (HR : R t' u')
+                      (Sbisimu : u' (~ LF) u),
+        @sbisim_clos_body LE LF R t u.
+
+  Program Definition sbisim_clos {LE LF} : mon (rel (ctree E X) (ctree F Y)) :=
+    {| body := @sbisim_clos_body LE LF |}.
+  Next Obligation. destruct H0; econstructor; eauto. Qed.
+
+  
+  (*| stuck ctrees can be simulated by anything. |*)
+  Lemma is_stuck_sb (R : rel _ _) (t : ctree E X) (t': ctree F Y):
+    is_stuck t -> is_stuck t' -> sb L R t t'.
+  Proof.
+    split; repeat intro; exfalso. 
+    - apply H; now (exists l, t'0).
+    - apply H0; now (exists l, t'0).
+  Qed.
+
+  Theorem sbisim_clos_upto R: @sbisim_clos eq eq R <= st L R.
+  Proof.
+    apply leq_t.
+    intros S t u HRel.
+    split; cbn; intros ? ? TR.
+    - inv HRel.
+      step in Sbisimt; apply Sbisimt in TR; destruct TR as (? & ? & TR & Sbis & <-).
+      apply HR in TR; destruct TR as (? & ? & TR & Sbis' & HL).
+      step in Sbisimu; apply Sbisimu in TR; destruct TR as (? & ? & TR & Sbis'' & <-).
+      do 2 eexists; repeat split; eauto.
+      econstructor.
+      apply Sbis.
+      eauto.
+      apply Sbis''.
+    - inv HRel.
+      step in Sbisimu; apply Sbisimu in TR; destruct TR as (? & ? & TR & Sbis & <-).
+      apply HR in TR; destruct TR as (? & ? & TR & Sbis' & HL).
+      step in Sbisimt; apply Sbisimt in TR; destruct TR as (? & ? & TR & Sbis'' & <-).
+      do 2 eexists; repeat split; eauto.
+      econstructor.
+      apply Sbis''.
+      eauto.
+      apply Sbis.
+  Qed.
+
+End sbisim_heterogenous_theory.
+
+Definition respects_val `{Encode E} `{Encode F} (L : rel (label E) (label F)) :=
+  forall l l', L l l' -> is_val l <-> is_val l'.
+
+Definition respects_tau `{Encode E} `{Encode F} (L : rel (label E) (label F)) :=
+  forall l l', L l l' -> l = tau <-> l' = tau.
+
+Definition eq_obs `{Encode E} (L : relation (label E)) : Prop :=
+  forall e e' (x : encode e) (x' : encode e'),
+    L (obs e x) (obs e' x') -> obs e x = obs e' x'.
+
+Lemma respects_val_eq `{Encode E}: respects_val (@eq (label E)).
+Proof.
+  split; intros; subst; auto. 
+Defined.
+
+Lemma respects_tau_eq `{Encode E}: respects_tau (@eq (label E)).
+Proof.
+  split; intros; subst; auto. 
+Defined.
+Global Hint Resolve respects_val_eq respects_tau_eq: ctree.
+
+Section sbisim_homogenous_theory.
+  Context {E: Type} {HE: Encode E} {X: Type} {L: relation (label E)}.
+
+  Local Notation sb  := (@sb E E HE HE X X).
+  Local Notation sbisim := (@sbisim E E HE HE X X).
+  Local Notation st L := (coinduction.t (sb L)).
+  Local Notation sbt L := (coinduction.bt (sb L)).
+  Local Notation sT  L := (coinduction.T (sb L)).
+
+  (*|
+    This is just a hack suggested by Damien Pous to avoid a
+    universe inconsistency when using both the relational algebra
+    and coinduction libraries (we fix the type at which we'll use [eq]). |*)
+
+  Lemma refl_st {RL: Reflexive L} : const eq <= (st L).
+  Proof.
+    apply leq_t.
+    split; intros; cbn*; intros; inv H; subst;
+      exists l, t'; split; eauto.
+  Qed.
+
+(*|
+[converse] is compatible
+i.e. validity of up-to symmetry
+|*)
+  Lemma converse_st `{SL: Symmetric _ L}: converse <= (st L).
+  Proof.
+    apply leq_t; cbn.
+    intros R ? ? [H1 H2]; split; intros.
+    - destruct (H2 _ _ H) as (? & ? & ? & ? & ?); subst; symmetry in H4; eauto.
+    - destruct (H1 _ _ H) as (? & ? & ? & ? & ?); subst; symmetry in H4; eauto.
+  Qed.
+
+(*|
+[square] is compatible
+i.e. validity of up-to transivitiy
+|*)
+  Lemma square_st `{TR: Transitive _ L}: square <= (st L).
+  Proof.
+    apply Coinduction; cbn.
+    intros R x z [y [xy yx] [yz zy]].
+    split.
+     - intros ?l x' xx'.
+      destruct (xy _ _ xx') as (?l & y' & yy' & ? & EQ).
+      destruct (yz _ _ yy') as (?l & z' & zz' & ? & EQ').
+      do 2 eexists; repeat split.
+      eauto.
+      apply (f_Tf (sb L)).
+      eexists; eauto.
+      transitivity l0; assumption.
+    - intros ?l z' zz'.
+      destruct (zy _ _ zz') as (?l & y' & yy' & ? & EQ).
+      destruct (yx _ _ yy') as (?l & x' & xx' & ? & EQ').
+      do 2 eexists; repeat split.
+      eauto.
+      apply (f_Tf (sb L)).
+      eexists; eauto.
+      transitivity l0; assumption.
+  Qed.
+
+(*|
+Reflexivity
+|*)
+  #[global] Instance Reflexive_st R `{Reflexive _ L}: Reflexive (st L R).
+  Proof. apply build_reflexive; apply ft_t; apply refl_st. Qed.
+
+  #[global] Instance Reflexive_sbisim `{Reflexive _ L}: Reflexive (sbisim L).
+  Proof. now apply Reflexive_st. Qed.
+
+  #[global] Instance Reflexive_sbt R `{Reflexive _ L}: Reflexive (sbt L R).
+  Proof. apply build_reflexive; apply fbt_bt; apply refl_st. Qed.
+
+  #[global] Instance Reflexive_sT f R `{Reflexive _ L}: Reflexive (sT L f R).
+  Proof. apply build_reflexive; apply fT_T; apply refl_st. Qed.
+
+(*|
+Transitivity
+|*)
+  #[global] Instance Transitive_st R `{Transitive _ L}: Transitive (st L R).
+  Proof. apply build_transitive; apply ft_t; apply (square_st). Qed.
+
+  #[global] Instance Transitive_sbisim `{Transitive _ L}: Transitive (sbisim L).
+  Proof. now apply Transitive_st. Qed.
+
+  #[global] Instance Transitive_sbt R `{Transitive _ L}: Transitive (sbt L R).
+  Proof. apply build_transitive; apply fbt_bt; apply square_st. Qed.
+
+  #[global] Instance Transitive_sT f R `{Transitive _ L}: Transitive (sT L f R).
+  Proof. apply build_transitive; apply fT_T; apply square_st. Qed.
+
+(*|
+Symmetry
+|*)
+  #[global] Instance Symmetric_st R `{Symmetric _ L}: Symmetric (st L R).
+  Proof. apply build_symmetric; apply ft_t; apply (converse_st). Qed.
+
+  #[global] Instance Symmetric_sbisim `{Symmetric _ L}: Symmetric (sbisim L).
+  Proof. now apply Symmetric_st. Qed.
+
+  #[global] Instance Symmetric_sbt R `{Symmetric _ L}: Symmetric (sbt L R).
+  Proof. apply build_symmetric; apply fbt_bt; apply converse_st. Qed.
+
+  #[global] Instance Symmetric_sT f R `{Symmetric _ L}: Symmetric (sT L f R).
+  Proof. apply build_symmetric; apply fT_T; apply converse_st. Qed.
+
+(*|
+Thus bisimilarity and [t R] are always equivalence relations.
+|*)
+  #[global] Instance Equivalence_st `{Equivalence _ L} R: Equivalence (st L R).
+  Proof. split; typeclasses eauto. Qed.
+
+  #[global] Instance Equivalence_bisim `{Equivalence _ L}: Equivalence (sbisim L).
+  Proof. split; typeclasses eauto. Qed.
+
+  #[global] Instance Equivalence_sbt `{Equivalence _ L} R: Equivalence (sbt L R).
+  Proof. split; typeclasses eauto. Qed.
+
+  #[global] Instance Equivalence_sT `{Equivalence _ L} f R: Equivalence ((T (sb L)) f R).
+  Proof. split; typeclasses eauto. Qed.
+
+(*|
+Aggressively providing instances for rewriting hopefully faster
+[sbisim] under all [sb]-related contexts (consequence of the transitivity
+of the companion).
+|*)
+  #[global] Instance sbisim_sbisim_closed_goal `{Transitive _ L} `{Symmetric _ L} :
+    Proper (sbisim L ==> sbisim L ==> flip impl) (sbisim L).
+  Proof.
+    repeat intro.
+    etransitivity; [etransitivity; eauto | symmetry; eassumption].
+  Qed.
+
+  #[global] Instance sbisim_sbisim_closed_ctx `{Transitive _ L} `{Symmetric _ L} :
+    Proper (sbisim L ==> sbisim L ==> impl) (sbisim L).
+  Proof.
+    repeat intro.
+    etransitivity; [symmetry; eassumption | etransitivity; eauto].
+  Qed.
+
+  #[global] Instance sbisim_clos_st_goal `{Equivalence _ L} R:
+    Proper (sbisim L ==> sbisim L ==> flip impl) (st L R).
+  Proof.
+    cbn; intros ? ? eq1 ? ? eq2 ?.
+    rewrite eq1, eq2.
+    auto.
+  Qed.
+
+  #[global] Instance sbisim_clos_st_ctx `{Equivalence _ L} R :
+    Proper (sbisim L ==> sbisim L ==> impl) (st L R).
+  Proof.
+    cbn; intros ? ? eq1 ? ? eq2 ?.
+    rewrite <- eq1, <- eq2.
+    auto.
+  Qed.
+
+  #[global] Instance sbisim_clos_sT_goal `{Equivalence _ L} R f :
+    Proper (sbisim L ==> sbisim L ==> flip impl) (sT L f R).
+  Proof.
+    cbn; intros ? ? eq1 ? ? eq2 ?.
+    rewrite eq1, eq2.
+    auto.
+  Qed.
+
+  #[global] Instance sbisim_clos_sT_ctx `{Equivalence _ L} R f :
+    Proper (sbisim L ==> sbisim L ==> impl) (sT L f R).
+  Proof.
+    cbn; intros ? ? eq1 ? ? eq2 ?.
+    rewrite <- eq1, <- eq2.
+    auto.
+  Qed.
+
+  #[global] Instance equ_sbt_closed_goal `{EqL: Equivalence _ L} R:
+    Proper (equ eq ==> equ eq ==> flip impl) (sbt L R).
+  Proof.
+    repeat intro. pose proof (gfp_bt (sb L) R).
+    etransitivity; [| etransitivity]; [ | apply H1 | ]; apply H2.
+    rewrite H; auto. rewrite H0; auto.
+  Qed.
+
+  #[global] Instance equ_sbt_closed_ctx `{EqL: Equivalence _ L} {R} :
+    Proper (equ eq ==> equ eq ==> impl) (sbt L R).
+  Proof.
+    repeat intro. pose proof (gfp_bt (sb L) R).
+    etransitivity; [| etransitivity]; [ | apply H1 | ]; apply H2.
+    rewrite H; auto. rewrite H0; auto.
+  Qed.
+
+End sbisim_homogenous_theory.
+
+
+(*|
+Up-to [bind] context bisimulations
+----------------------------------
+We have proved in the module [Equ] that up-to bind context is
+a valid enhancement to prove [equ].
+We now prove the same result, but for strong and weak bisimulation.
+|*)
+
+Section bind.
+  Obligation Tactic := trivial.
+  Context {E F: Type} {HE: Encode E} {HF: Encode F} {X X' Y Y': Type}
+    {L: rel (label E) (label F)} (R0 : rel X Y).
+
+  Program Definition bind_ctx_sbisim L0 : mon (rel (ctree E X') (ctree F Y')) :=
+    {|body := fun R => @bind_ctx E F HE HF X Y X' Y' (sbisim L0)
+                              (pointwise R0 R) |}.
+  Next Obligation.
+    intros ??? H. apply leq_bind_ctx. intros ?? H' ?? H''.
+    apply in_bind_ctx. apply H'. intros t t' HS. apply H, H'', HS.
+  Qed.
+
+(*|
+The resulting enhancing function gives a valid up-to technique
+|*)
+  Lemma bind_ctx_sbisim_t L0 :
+    is_update_val_rel L R0 L0 -> bind_ctx_sbisim L0 <= st L.
+  Proof.
+    intros HL0. apply Coinduction.
+    intros R. apply (leq_bind_ctx _).
+    intros t1 t2 tt k1 k2 kk.
+    step in tt; split; simpl;  intros l u STEP.
+    - apply trans_bind_inv in STEP as [(VAL & t' & STEP & EQ) | (v & STEPres & STEP)]; cbn in *.
+      + apply tt in STEP as (l' & u' & STEP & SIM & LBL).
+        apply HL0 in LBL; etrans.
+        apply update_val_rel_nonval_l in LBL as [VAL' LBL]; auto.
+        do 2 eexists. split.
+        apply trans_bind_l; eauto.
+        split; auto.
+        apply (fT_T equ_clos_st).
+        econstructor; [exact EQ | | reflexivity].
+        apply (fTf_Tf (sb L)).
+        apply in_bind_ctx; auto.
+        intros ? ? ?.
+        apply (b_T (sb L)).
+        red in kk; now apply kk.
+      + apply tt in STEPres as (l' & u' & STEPres & SIM & LBL).
+        apply HL0 in LBL; etrans.
+        apply update_val_rel_val_l in LBL as (v' & -> & ?).
+        pose proof (trans_val_inv STEPres) as EQ.
+        rewrite <- EQ in STEPres.
+        specialize (kk v v' H).
+        apply kk in STEP as (l' & u'' & STEP & EQ'' & ?); cbn in *.
+        do 2 eexists; split.
+        eapply trans_bind_r; eauto.
+        split; auto.
+        eapply (id_T (sb L)); auto.
+    - apply trans_bind_inv in STEP as [(H & t' & STEP & EQ) | (v & STEPres & STEP)]; cbn in *.
+      + apply tt in STEP as (l' & u' & STEP & EQ' & LBL).
+        apply HL0 in LBL; etrans.
+        apply update_val_rel_nonval_r in LBL as [VAL' LBL]; auto.
+        do 2 eexists; split.
+        apply trans_bind_l; eauto.
+        split; auto.
+        apply (fT_T equ_clos_st).
+        symmetry in EQ.
+        econstructor; [reflexivity | | exact EQ].
+        apply (fTf_Tf (sb L)).
+        apply in_bind_ctx; auto.
+        intros ? ? ?.
+        apply (b_T (sb L)).
+        red in kk; now apply kk.
+      + apply tt in STEPres as (l' & u' & STEPres & EQ' & LBL).
+        apply HL0 in LBL; etrans.
+        apply update_val_rel_val_r in LBL as (v' & -> & ?).
+        pose proof (trans_val_inv STEPres) as EQ.
+        rewrite <- EQ in STEPres.
+        specialize (kk v' v H).
+        apply kk in STEP as (u'' & ? & STEP & EQ'' & ?); cbn in *.
+        do 2 eexists; split.
+        eapply trans_bind_r; eauto.
+        split; auto.
+        eapply (id_T (sb L)); auto.
+  Qed.
+
+End bind.
+
+Import Ctree.
+Import CTreeNotations.
+
+(*|
+Expliciting the reasoning rule provided by the up-to principles.
+This principle is unusable for most [L], see https://github.com/vellvm/ctrees/issues/21
+|*)
+Lemma st_clo_bind_gen {E F: Type} {HE: Encode E} {HF: Encode F} {X Y X' Y': Type}
+  {L : rel (label E) (label F)}
+  (R0 : rel X Y) L0
+  (t1 : ctree E X) (t2: ctree F Y)
+  (HL0 : is_update_val_rel L R0 L0)
+  (k1 : X -> ctree E X') (k2 : Y -> ctree F Y') RR:
+  t1 (~L0) t2 ->
+  (forall x y, R0 x y -> (st L RR) (k1 x) (k2 y)) ->
+  st L RR (t1 >>= k1) (t2 >>= k2).
+Proof.
+  intros ? ?.
+  apply (ft_t (@bind_ctx_sbisim_t E F HE HF X X' Y Y' L R0 L0 HL0)).
+  apply in_bind_ctx; eauto.
+Qed.
+
+Lemma st_clo_bind {E F: Type} {HE: Encode E} {HF: Encode F} {X Y X' Y': Type}
+  {L : rel (label E) (label F)}
+  (R0 : rel X Y)
+  (t1 : ctree E X) (t2: ctree F Y)
+  (k1 : X -> ctree E X') (k2 : Y -> ctree F Y') RR:
+  t1 (~update_val_rel L R0) t2 ->
+  (forall x y, R0 x y -> (st L RR) (k1 x) (k2 y)) ->
+  st L RR (t1 >>= k1) (t2 >>= k2).
+Proof.
+  intros ? ?.
+  eapply st_clo_bind_gen; eauto.
+  apply update_val_rel_correct.
+Qed.
+
+Lemma st_clo_bind_eq {E: Type} {HE: Encode E} {X X': Type}
+      (t1 : ctree E X) (t2: ctree E X)
+      (k1 : X -> ctree E X') (k2 : X -> ctree E X') RR:
+  t1 ~ t2 ->
+  (forall x, st eq RR (k1 x) (k2 x)) ->
+  st eq RR (t1 >>= k1) (t2 >>= k2).
+Proof.
+  intros ? ?.
+  eapply st_clo_bind_gen.
+  - apply is_update_val_rel_eq.
+  - assumption.
+  - intros. now subst.
+Qed.
+
+Lemma sbt_clo_bind_gen `{HE: Encode E} `{HF: Encode F} {X Y X' Y': Type} {L : rel (label E) (label F)}
+      (R0 : rel X Y) L0
+      (t1 : ctree E X) (t2: ctree F Y)
+      (HL0 : is_update_val_rel L R0 L0)
+      (k1 : X -> ctree E X') (k2 : Y -> ctree F Y') RR:
+  t1 (~L0) t2 ->
+  (forall x y, R0 x y -> (sbt L RR) (k1 x) (k2 y)) ->
+  sbt L RR (t1 >>= k1) (t2 >>= k2).
+Proof.
+  intros ? ?.
+  apply (fbt_bt (@bind_ctx_sbisim_t E F HE HF X X' Y Y' L R0 L0 HL0)).
+  apply in_bind_ctx; eauto.
+Qed.
+
+Lemma sbt_clo_bind {E F: Type} `{HE: Encode E} `{HF: Encode F} {X Y X' Y': Type}
+  {L : rel (label E) (label F)}
+      (R0 : rel X Y)
+      (t1 : ctree E X) (t2: ctree F Y)
+      (k1 : X -> ctree E X') (k2 : Y -> ctree F Y') RR:
+  t1 (~update_val_rel L R0) t2 ->
+  (forall x y, R0 x y -> (sbt L RR) (k1 x) (k2 y)) ->
+  sbt L RR (t1 >>= k1) (t2 >>= k2).
+Proof.
+  intros ? ?.
+  eapply sbt_clo_bind_gen; eauto.
+  apply update_val_rel_correct.
+Qed.
+
+Lemma sbt_clo_bind_eq `{HE: Encode E} {X X': Type}
+      (t1 : ctree E X) (t2: ctree E X)
+      (k1 : X -> ctree E X') (k2 : X -> ctree E X') RR:
+  t1 ~ t2 ->
+  (forall x, sbt eq RR (k1 x) (k2 x)) ->
+  sbt eq RR (t1 >>= k1) (t2 >>= k2).
+Proof.
+  intros ? ?.
+  eapply sbt_clo_bind_gen.
+  - apply is_update_val_rel_eq.
+  - assumption.
+  - intros. now subst.
+Qed.
+
+Lemma sbisim_clo_bind_gen `{HE: Encode E} `{HF: Encode F} {X Y X' Y': Type} {L : rel (label E) (label F)}
+      (R0 : rel X Y) L0
+      (t1 : ctree E X) (t2: ctree F Y)
+      (HL0 : is_update_val_rel L R0 L0)
+      (k1 : X -> ctree E X') (k2 : Y -> ctree F Y') :
+  t1 (~L0) t2 ->
+  (forall x y, R0 x y -> k1 x (~L) k2 y) ->
+  t1 >>= k1 (~L) t2 >>= k2.
+Proof.
+  now apply st_clo_bind_gen.
+Qed.
+
+Lemma sbisim_clo_bind `{HE: Encode E} `{HF: Encode F} {X Y X' Y': Type}
+  {L : rel (label E) (label F)}
+  (R0 : rel X Y)
+  (t1 : ctree E X) (t2: ctree F Y)
+  (k1 : X -> ctree E X') (k2 : Y -> ctree F Y') :
+  t1 (~update_val_rel L R0) t2 ->
+  (forall x y, R0 x y -> k1 x (~L) k2 y) ->
+  t1 >>= k1 (~L) t2 >>= k2.
+Proof. now apply st_clo_bind. Qed.
+
+Lemma sbisim_clo_bind_eq `{HE: Encode E} {X X': Type}
+      (t1 : ctree E X) (t2: ctree E X)
+      (k1 : X -> ctree E X') (k2 : X -> ctree E X') :
+  t1 ~ t2 ->
+  (forall x, k1 x ~ k2 x) ->
+  t1 >>= k1 ~ t2 >>= k2.
+Proof. now apply st_clo_bind_eq. Qed.
+
+(*|
+And in particular, we get the proper instance justifying rewriting [~] to the left of a [bind].
+|*)
+#[global] Instance bind_sbisim_cong_gen `{HE: Encode E} {X X'} (RR: relation (ctree E X')):
+  Proper (sbisim eq ==> pointwise_relation X (st eq RR) ==> st eq RR) (@bind E HE X X').
+Proof.
+  unfold Proper, respectful, pointwise_relation.
+  intros.
+  now apply st_clo_bind_eq.
+Qed.
+
+Ltac __upto_bind_sbisim :=
+  match goal with
+    |- @sbisim ?E ?F ?C ?D ?X ?Y ?L
+              (Ctree.bind (X := ?T) _ _) (Ctree.bind (X := ?T) _ _) => apply sbisim_clo_bind_eq
+  | |- body (t (@sb ?E ?F ?C ?D ?X ?Y ?L)) ?R
+           (Ctree.bind (X := ?X') _ _) (Ctree.bind (X := ?X') _ _) =>
+      apply st_clo_bind_eq
+  | |- body (bt (@sb ?E ?F ?C ?D ?X ?Y ?L)) ?R
+           (Ctree.bind (X := ?X') _ _) (Ctree.bind (X := ?X') _ _) =>
+      apply sbt_clo_bind_eq
+  end.
+
+Ltac __upto_bind_eq_sbisim :=
+  match goal with
+  | |- @sbisim ?E ?F ?C ?D ?X ?Y eq (Ctree.bind (X := ?Z) _ _) (Ctree.bind (X := ?Z) _ _) =>
+      __upto_bind_sbisim; [reflexivity | intros ?]
+  | _ =>
+      __upto_bind_sbisim; [reflexivity | intros ? ? EQl]
+  end.
+
+Section Ctx.
+
+  Context {E F: Type} {HE: Encode E} {HF: Encode F} {X X' Y Y': Type}.
+
+  Definition vis_ctx (e : E) (f: F)
+             (R: rel (encode e -> ctree E X') (encode f -> ctree F Y')):
+    rel (ctree E X') (ctree F Y') :=
+    sup_all (fun k => sup (R k) (fun k' => pairH (Vis e k) (Vis f k'))).
+  
+  Lemma leq_vis_ctx (e: E) (f: F):
+    forall (R: rel (encode e -> ctree E X') (encode f -> ctree F Y')) R', vis_ctx R <= R' <->
+              (forall k k', R k k' -> R' (Vis e k) (Vis f k')).
+  Proof.
+    intros.
+    unfold vis_ctx.
+    setoid_rewrite sup_all_spec.
+    setoid_rewrite sup_spec.
+    setoid_rewrite <-leq_pairH.
+    firstorder.
+  Qed.
+
+  Lemma in_vis_ctx e f (R :rel _ _) x x' :
+    R x x' -> vis_ctx R (Vis e x) (Vis f x').
+  Proof. intros. now apply ->leq_vis_ctx. Qed.
+  #[global] Opaque vis_ctx.
+
+End Ctx.
+
+Section sb_vis_ctx.
+
+  Obligation Tactic := idtac.
+
+  Section Gen.
+    Context {E F: Type} {HE: Encode E} {HF: Encode F} {X Y X' Y': Type}.
+
+    Program Definition vis_ctx_sbisim_gen (e : E) (f: F)
+      (right : encode e -> encode f) (left : encode f -> encode e) :
+      mon (rel (ctree E X') (ctree F Y')) :=
+      {|body := fun R =>
+                  @vis_ctx E F HE HF X' Y' e f
+                    (fun ff gg =>
+                       (forall x, R (ff x) (gg (right x))) /\
+                         (forall y, R (ff (left y)) (gg y)))
+      |}.
+    Next Obligation.
+      intros e f Rf Rg ? ? ? . apply leq_vis_ctx. intros k k' [H1 H2].
+      apply in_vis_ctx; split; intros.
+      eapply H in H1; eapply H1.
+      eapply H in H2; eapply H2.
+    Qed.
+
+    (*| The resulting enhancing function gives a valid up-to technique |*)
+    Lemma vis_ctx_sbisim_gen_t {L: rel (label E) (label F)} (e : E) (f: F)
+      (right: encode e -> encode f) (left: encode f -> encode e) :
+      (forall x, L (obs e x) (obs f (right x))) ->
+      (forall y, L (obs e (left y)) (obs f y)) ->
+      vis_ctx_sbisim_gen right left <= (st L).
+    Proof.
+      intros HHT HHF.
+      apply Coinduction.
+      intros R.
+      apply leq_vis_ctx.
+      intros k k' kk'.
+      cbn.
+      split; intros ? ? TR; trans in TR; cbn.
+      - do 2 eexists; split; etrans; split; auto.
+        rewrite Eqt; now eapply (b_T (sb L)).
+      - do 2 eexists; split; etrans; split; auto.
+        rewrite Eqt; now eapply (b_T (sb L)).
+    Qed.
+
+  End Gen.
+
+  Section Specialized.
+
+    Context {E: Type} `{HE: Encode E} {X X': Type}.
+
+    Program Definition vis_ctx_sbisim (e : E) :
+      mon (rel (ctree E X') (ctree E X')) :=
+      {|body := fun R =>
+                  @vis_ctx E E HE HE X' X' e e
+                    (fun ff gg => forall x, R (ff x) (gg x))
+      |}.
+    Next Obligation.
+      intros e ? ? ?. apply leq_vis_ctx. intros k k' H0.
+      apply in_vis_ctx; intros.
+      eapply H in H0; eapply H0.
+    Qed.
+
+(*|
+The resulting enhancing function gives a valid up-to technique
+|*)
+    Lemma vis_ctx_sbisim_t (e : E) :
+      vis_ctx_sbisim e <= (st eq).
+    Proof.
+      apply Coinduction.
+      intros R.
+      apply leq_vis_ctx.
+      intros k k' kk'.
+      cbn.
+      split; intros ? ? TR; trans in TR; subst; cbn.
+      - do 2 eexists; split; etrans; split; auto.
+        rewrite Eqt; now eapply (b_T (sb eq)).
+      - do 2 eexists; split; etrans; split; auto.
+        rewrite Eqt; now eapply (b_T (sb eq)).
+    Qed.
+
+  End Specialized.
+
+End sb_vis_ctx.
+
+Arguments vis_ctx_sbisim_t {E HE X'} e.
+
+Ltac __upto_vis_sbisim :=
+  match goal with
+    |- @sbisim ?E ?F ?HE ?HF ?X _ ?RR (Vis ?e _) (Vis ?e _) =>
+      apply (ft_t (vis_ctx_sbisim_t e)), in_vis_ctx; intros ?
+  | |- body (t (@sb ?E ?F ?HE ?HF ?X _ _ ?R _)) ?RR (Vis ?e _) (Vis ?f _) =>
+      apply (ft_t (vis_ctx_sbisim_t e)), in_vis_ctx; intros ?
+  | |- body (bt (@sb ?E ?F ?C _ ?X _ _ ?R _)) ?RR (Vis ?e _) (Vis ?f _) =>
+      apply (fbt_bt (vis_ctx_sbisim_t e)), in_vis_ctx; intros ?
+  end.
+
+#[local] Tactic Notation "upto_vis" := __upto_vis_sbisim.
+
+Ltac __play_sbisim := step; split; cbn; intros ? ? ?TR.
+
+Ltac __playL_sbisim H :=
+  step in H;
+  let Hf := fresh "Hf" in
+  destruct H as [Hf _];
+  cbn in Hf; edestruct Hf as (? & ? & ?TR & ?EQ & ?);
+  clear Hf; subst; [etrans |].
+
+Ltac __eplayL_sbisim :=
+  match goal with
+  | h : @sbisim ?E ?F _ _ ?X ?Y ?L _ _ |- _ =>
+      __playL_sbisim h
+  end.
+
+Ltac __playR_sbisim H :=
+  step in H;
+  let Hb := fresh "Hb" in
+  destruct H as [_ Hb];
+  cbn in Hb; edestruct Hb as (? & ? & ?TR & ?EQ & ?);
+  clear Hb; subst; [etrans |].
+
+Ltac __eplayR_sbisim :=
+  match goal with
+  | h : @sbisim ?E ?F ?HE ?HF ?X ?Y ?L _ _ |- _ =>
+      __playR_sbisim h
+  end.
+
+#[local] Tactic Notation "play" := __play_sbisim.
+#[local] Tactic Notation "playL" "in" ident(H) := __playL_sbisim H.
+#[local] Tactic Notation "playR" "in" ident(H) := __playR_sbisim H.
+#[local] Tactic Notation "eplayL" := __eplayL_sbisim.
+#[local] Tactic Notation "eplayR" := __eplayR_sbisim.
+
+(*|
+Proof rules for [~]
+-------------------
+Naive bisimulations proofs naturally degenerate into exponential proofs,
+splitting into two goals at each step.
+The following proof rules avoid this issue in particular cases.
+
+Be sure to notice that contrary to equations such that [sb_guard] or
+up-to principles such that [upto_vis], (most of) these rules consume a [sb].
+
+TODO: need to think more about this --- do we want more proof rules?
+Do we actually need them on [sb (st R)], or something else?
+|*)
+Section Proof_Rules.
+  Context {E F: Type} {HE: Encode E} {HF: Encode F} {X Y: Type} {L: rel (label E) (label F)}.
+
+  Lemma step_sb_ret_gen(x: X) (y: Y) (R : rel (ctree E X) (ctree F Y)) :
+    R stuck stuck ->
+    L (val x) (val y) ->
+    (Proper (equ eq ==> equ eq ==> impl) R) ->
+    sb L R (Ret x) (Ret y).
+  Proof.
+    intros Rstuck ValRefl PROP.
+    split; apply step_ss_ret_gen; eauto.
+    typeclasses eauto.
+  Qed.
+  
+  Lemma step_sb_ret (x: X) (y: Y) (R : rel (ctree E X) (ctree F Y)) :
+    L (val x) (val y) ->
+    sbt L R (Ret x) (Ret y).
+  Proof.
+    intros LH; subst.
+    apply step_sb_ret_gen; eauto.
+    - step; split;
+      apply is_stuck_sb; apply stuck_is_stuck.
+    - typeclasses eauto.
+  Qed.
+
+  (*|
+    The vis nodes are deterministic from the perspective of the labeled transition system,
+    stepping is hence symmetric and we can just recover the itree-style rule.
+  |*)
+  Lemma step_sb_vis_gen {X' Y'} (e: E) (f: F)
+    (k: encode e -> ctree E X') (k': encode f -> ctree F Y') {R : rel _ _}:
+    (Proper (equ eq ==> equ eq ==> impl) R) ->
+    (forall x, exists y, R (k x) (k' y) /\ L (obs e x) (obs f y)) ->
+    (forall y, exists x, R (k x) (k' y) /\ L (obs e x) (obs f y)) ->
+    sb L R (Vis e k) (Vis f k').
+  Proof.
+    intros PR EQs EQs'.
+    split; apply step_ss_vis_gen; eauto.
+    typeclasses eauto.
+  Qed.
+
+  Lemma step_sb_vis {X' Y'} (e: E) (f: F) (k: encode e -> ctree E X') (k': encode f -> ctree F Y') {R : rel _ _}:
+    (forall x, exists y, st L R (k x) (k' y) /\ L (obs e x) (obs f y)) ->
+    (forall y, exists x, st L R (k x) (k' y) /\ L (obs e x) (obs f y)) ->
+    sbt L R (Vis e k) (Vis f k').
+  Proof.
+    intros EQs EQs'.
+    apply step_sb_vis_gen; eauto.
+    typeclasses eauto.
+  Qed.
+
+  (*| Same goes for visible tau nodes. |*)
+  Lemma step_sb_step_gen (t : ctree E X) (t' : ctree F Y) (R: rel _ _) :
+    (Proper (equ eq ==> equ eq ==> impl) R) ->
+    L tau tau ->
+    (R t t') ->
+    sb L R (step t) (step t').
+  Proof.
+    intros. split; apply step_ss_step_gen; auto.
+    typeclasses eauto.
+  Qed.
+
+  Lemma step_sb_step (t : ctree E X) (t' : ctree F Y) (R: rel _ _) :
+    L tau tau ->
+    (st L R t t') ->
+    sbt L R (step t) (step t').
+  Proof.
+    apply step_sb_step_gen.
+    typeclasses eauto.
+  Qed.
+
+  Lemma step_sb_br_gen {n m}
+    (k : fin' n -> ctree E X) (k': fin' m  -> ctree F Y) (R : rel _ _):
+    (Proper (equ eq ==> equ eq ==> impl) R) ->
+    L tau tau ->
+    (forall x, exists y, R (k x) (k' y)) ->
+    (forall y, exists x, R (k x) (k' y)) ->
+    sb L R (Br n k) (Br m k').
+  Proof.
+    intros PROP ? EQs1 EQs2.
+    split; intros ? ? TR; trans in TR. 
+    - destruct (EQs1 n0) as [y HR].
+      exists tau, (k' y); split; [etrans|].
+      rewrite Eqt; auto.
+    - destruct (EQs2 n0) as [y HR].
+      exists tau, (k y); split; [etrans|].
+      rewrite Eqt; auto.
+  Qed.
+
+  Lemma step_sb_br {n m}
+    (k : fin' n -> ctree E X) (k': fin' m  -> ctree F Y) (R : rel _ _):
+    L tau tau ->
+    (forall x, exists y, st L R (k x) (k' y)) ->
+    (forall y, exists x, st L R (k x) (k' y)) ->
+    sbt L R (Br n k) (Br m k').
+  Proof.
+    intros EQs1 EQs2.
+    apply step_sb_br_gen; auto.
+    typeclasses eauto.
+  Qed.
+
+  Lemma step_sb_br_id_gen {n} 
+        (k : fin' n -> ctree E X) (k': fin' n -> ctree F Y) (R: rel _ _) :
+    (Proper (equ eq ==> equ eq ==> impl) R) ->
+    L tau tau ->
+    (forall x, R (k x) (k' x)) ->
+    sb L R (Br n k) (Br n k').
+  Proof.
+    intros PROP ? EQs.
+    apply step_sb_br_gen; trivial; intros x; exists x; auto.
+  Qed.
+
+  Lemma step_sb_br_id {n} 
+    (k : fin' n -> ctree E X) (k': fin' n -> ctree F Y) (R: rel _ _) :
+    L tau tau ->
+    (forall x, st L R (k x) (k' x)) ->
+    sbt L R (Br n k) (Br n k').
+  Proof.
+    apply step_sb_br_id_gen.
+    typeclasses eauto.
+  Qed.
+
+  (*|
+    For invisible nodes, the situation is different: we may kill them, but that execution
+    cannot act as going under the guard.
+  |*)
+  Lemma step_sb_guard_gen (t : ctree E X) (t': ctree F Y) (R: rel _ _) :
+    sb L R t t' ->
+    sb L R (Guard t) (Guard t').
+  Proof.
+    intros EQ.
+    split; apply step_ss_guard_gen; apply EQ.
+  Qed.
+
+  Lemma step_sb_guard (t : ctree E X) (t' : ctree F Y) (R: rel _ _) :
+    sbt L R t t' ->
+    sbt L R (Guard t) (Guard t').
+  Proof.
+    now apply step_sb_guard_gen.
+  Qed.
+
+End Proof_Rules.
+
+(*|
+Proof system for homogenous [~]
+--------------------
+
+While the proof rules from the previous section are useful for performing full on
+coinductive proofs, lifting these at the level of [sbisim] can allow for completely
+avoiding any coinduction when combined with a pre-established equational theory.
+|*)
+Section Sb_Proof_System.
+  Context {E: Type} {HE: Encode E} {X: Type}.
+
+  Lemma sb_ret: forall x y,
+      x = y ->
+      (Ret x: ctree E X) ~ Ret y.
+  Proof.
+    intros * EQ; step.
+    now apply step_sb_ret; subst.
+  Qed.
+
+  Lemma sb_vis {Y}: forall (e: E) (k k': encode e -> ctree E Y),
+      (forall x, k x ~ k' x) ->
+      Vis e k ~ Vis e k'.
+  Proof.
+    intros.
+    upto_vis.
+    apply H.
+  Qed.
+
+  (*|
+    Visible vs. Invisible Taus
+    ~~~~~~~~~~~~~~~~~~~~~~~~~~
+    Invisible taus can be stripped-out w.r.t. to [sbisim], but not visible ones
+  |*)
+  Lemma sb_guard: forall (t : ctree E X),
+      Guard t ~ t.
+  Proof.
+    intros t; play.
+    - trans in TR; etrans. 
+    - eauto 6 with trans.
+  Qed.
+
+ Lemma sb_guard_l: forall (t u : ctree E X),
+      t ~ u ->
+      Guard t ~ u.
+  Proof.
+    intros * EQ; now rewrite sb_guard.
+  Qed.
+
+  Lemma sb_guard_r: forall (t u : ctree E X),
+      t ~ u ->
+      t ~ Guard u.
+  Proof.
+    intros * EQ; now rewrite sb_guard.
+  Qed.
+
+  Lemma sb_guard_lr: forall (t u : ctree E X),
+      t ~ u ->
+      Guard t ~ Guard u.
+  Proof.
+    intros * EQ; now rewrite !sb_guard.
+  Qed.
+  
+  Lemma sb_step: forall (t u : ctree E X),
+      t ~ u ->
+      step t ~ step u.
+  Proof.
+    intros * EQ; step.
+    apply step_sb_step; auto.
+  Qed.
+
+  Lemma sb_br {n m} (k : fin' n -> ctree E X) (k': fin' m -> ctree E X) :
+    (forall x, exists y, k x ~ k' y) ->
+    (forall y, exists x, k x ~ k' y) ->
+    Br n k ~ Br m k'.
+  Proof.
+    intros * EQs1 EQs2; step.
+    apply @step_sb_br; auto.
+  Qed.
+
+  Lemma sb_br_id {n} (k k' : fin' n -> ctree E X) :
+    (forall x, k x ~ k' x) ->
+    Br n k ~ Br n k'.
+  Proof.
+    intros * EQs; step.
+    apply @step_sb_br_id; auto.
+  Qed.
+
+  Lemma sb_unfold_forever: forall (k: X -> ctree E X)(i: X),
+      forever k i ~ r <- k i ;; forever k r.
+  Proof.
+    intros k i.
+    rewrite (ctree_eta (forever k i)).
+    unfold forever, Classes.iter, MonadIter_ctree.    
+    cbn.
+    rewrite <- ctree_eta.
+    rewrite unfold_iter, bind_map.
+    __upto_bind_eq_sbisim.
+    apply sb_guard.
+  Qed.
+
+  Lemma sb_unfold_iter{I}: forall (step: I -> ctree E (I + X))(i: I),
+      iter step i ~
+        (lr <- step i;;
+         match lr with
+         | inl l => iter step l
+         | inr r => Ret r
+         end).
+  Proof.
+    intros step i.
+    rewrite unfold_iter.
+    __upto_bind_eq_sbisim.
+    destruct x.
+    - apply sb_guard.
+    - reflexivity.
+  Qed.
+
+End Sb_Proof_System.
+
+(* TODO: tactics!
+   Should it be the same to step at both levels or two different sets?
+
+Ltac bsret  := apply step_sb_ret.
+Ltac bsvis  := apply step_sb_vis.
+Ltac bstauv := apply step_sb_tauV.
+Ltac bsstep := bsret || bsvis || bstauv.
+
+Ltac sret  := apply sb_ret.
+Ltac svis  := apply sb_vis.
+Ltac stauv := apply sb_tauV.
+Ltac sstep := sret || svis || stauv.
+ *)
+
+Section SanityChecks.
+  Context {E: Type} {HE: Encode E} {X: Type}.
+
+  Lemma sbisim_ret_inv (r1 r2 : X) :
+    (Ret r1 : ctree E X) ~ Ret r2 -> r1 = r2.
+  Proof.
+    intro.
+    eplayL.    
+    trans in TR.
+    dependent destruction Eql.
+    reflexivity.
+  Qed.
+
+  (*| Need to know [encode e1] is inhabited to take a step (not [void]) |*)
+  Lemma sbisim_vis_invT {e1 e2: E} {k1: encode e1 -> ctree E X} {k2: encode e2 -> ctree E X} (x: encode e1):
+    Vis e1 k1 ~ Vis e2 k2 ->
+    encode e1 = encode e2 /\ e1 = e2.
+  Proof.
+    intros Hsim.
+    eplayL.
+    trans in TR.
+    dependent destruction Eql.
+    auto.
+    Unshelve. exact x.
+  Qed.
+
+  Lemma sbisim_vis_invE (e: E) (k1 k2: encode e -> ctree E X) (x: encode e):
+    Vis e k1 ~ Vis e k2 ->
+    forall x, k1 x ~ k2 x.
+  Proof.
+    intros.
+    eplayL.
+    trans in TR.
+    dependent destruction Eql.
+    rewrite <- Eqt.
+    apply EQ.
+  Qed.
+
+  Lemma sbisim_br_inv {Y n m} (k1 : fin' n -> ctree E X) (k2: fin' m -> ctree E Y) :
+    Br n k1 ~ Br m k2 ->
+    (forall i1, exists i2, k1 i1 ~ k2 i2).
+  Proof.
+    intros EQ i1.
+    eplayL.
+    trans in TR.
+    exists n0; rewrite <- Eqt.
+    apply EQ.
+  Qed.
+
+  Lemma sbisim_ret_vis_inv (r : X) (e : E) (k : encode e -> ctree E X) :
+    Ret r ~ Vis e k -> False.
+  Proof.
+    intros * abs.
+    eplayL.
+    unfold trans in TR; cbn in TR.
+    inversion TR.
+  Qed.
+
+  Lemma sbisim_ret_br_inv {n} (r: X) (k : fin' n -> ctree E X) :
+    Ret r ~ Br n k -> False.
+  Proof.
+    intros * abs.
+    eplayL.
+    unfold trans in TR; cbn in TR.
+    inversion TR.
+  Qed.
+
+  Lemma sbisim_vis_br_inv{n} (e: E) (k1 : encode e -> ctree E X) (k2: fin' n -> ctree E X):
+    Vis e k1 ~ Br n k2 -> False.
+  Proof.
+    intros * abs.
+    eplayR.
+    inversion TR.
+    Unshelve. exact Fin.F1. 
+  Qed.
+  
+End SanityChecks.
+
+Section StrongSimulations.
+
+  Context {E F: Type} {HE: Encode E} {HF: Encode F} {X Y: Type}
+          {L: rel (label E) (label F)}.
+
+  Notation ss := (@ss E F HE HF X Y).
+  Notation sst L := (coinduction.t (ss L)).
+  Notation ssim  := (@ssim E F HE HF X Y).
+  Notation ssbt L := (coinduction.bt (ss L)).
+  Notation ssT L := (coinduction.T (ss L)).
+
+  Lemma sbisim_clos_ss : @sbisim_clos E HE F HF X Y eq eq <= (sst L).
+  Proof.
+    intro R1. apply Coinduction.
+    cbn; intros Rs x y [z x' y' z' SBzx' x'y' SBy'z'].
+    - intros l t zt.
+      step in SBzx'.
+      apply SBzx' in zt as (l' & t' & x't' & ? & ?); subst.
+      destruct (x'y' _ _ x't') as (l'' & t'' & y't'' & ? & ?).
+      step in SBy'z'.
+      apply SBy'z' in y't'' as (ll & tt & z'tt & ? & ?); subst.
+      exists ll, tt; split; trivial.
+      + split; trivial.
+        apply (f_Tf (ss L)).
+        econstructor; eauto.
+  Qed.
+
+  (*| Instances for rewriting [sbisim] under all [ss]-related contexts |*)
+  #[global] Instance sbisim_eq_clos_ssim_goal:
+    Proper (sbisim eq ==> sbisim eq ==> flip impl) (ssim L).
+  Proof.
+    cbn.
+    coinduction R CH. intros * EQ1 * EQ2 SIM.
+    do 2 red; cbn; intros * TR.
+    symmetry in EQ2.
+    step in EQ1; apply EQ1 in TR as (? & ? & ? & ? & ?).
+    step in SIM; apply SIM in H as (? & ? & ? & ? & ?).
+    step in EQ2; apply EQ2 in H as (? & ? & ? & ? & ?); subst.
+    do 2 eexists.
+    split; [eassumption |].
+    split; [| eassumption].
+    symmetry in H4. eapply CH; eassumption.
+  Qed.
+
+  #[global] Instance sbisim_eq_clos_ssim_ctx :
+    Proper (sbisim eq ==> sbisim eq ==> impl) (ssim L).
+  Proof.
+    repeat intro. symmetry in H, H0. eapply sbisim_eq_clos_ssim_goal; eauto.
+  Qed.
+
+  #[global] Instance sbisim_eq_clos_sst_goal RR :
+    Proper (sbisim eq ==> sbisim eq ==> flip impl) (sst L RR).
+  Proof.
+    cbn; intros ? ? eq1 ? ? eq2 H.
+    apply (ft_t sbisim_clos_ss). cbn.
+    econstructor; eauto.
+    now rewrite eq2.
+  Qed.
+
+  #[global] Instance sbisim_eq_clos_sst_ctx RR :
+    Proper (sbisim eq ==> sbisim eq ==> impl) (sst L RR).
+  Proof.
+    cbn; intros ? ? eq1 ? ? eq2 ?.
+    rewrite <- eq1, <- eq2.
+    auto.
+  Qed.
+
+  #[global] Instance sbisim_eq_clos_ssT_goal RR f :
+    Proper (sbisim eq ==> sbisim eq ==> flip impl) (ssT L f RR).
+  Proof.
+    cbn; intros ? ? eq1 ? ? eq2 H.
+    apply (fT_T sbisim_clos_ss). cbn.
+    econstructor; eauto.
+    now rewrite eq2.
+  Qed.
+
+  #[global] Instance sbisim_eq_clos_ssT_ctx RR f :
+    Proper (sbisim eq ==> sbisim eq ==> impl) (ssT L f RR).
+  Proof.
+    cbn; intros ? ? eq1 ? ? eq2 ?.
+    rewrite <- eq1, <- eq2.
+    auto.
+  Qed.
+
+End StrongSimulations.
