theories/CTree/SBisim/SSim.v
@@ -1,0 +1,908 @@
+From Coq Require Import
+     Lia
+     Basics
+     Fin
+     RelationClasses
+     Program.Equality
+     Logic.Eqdep.
+
+From Coinduction Require Import
+     coinduction rel tactics.
+
+From CTree Require Import
+  Events.Core
+  CTree.Core
+  CTree.Equ
+  CTree.Trans.
+
+Import Ctree.
+Local Open Scope ctree_scope.
+Set Implicit Arguments.
+Generalizable All Variables.
+
+(* TODO: Decide where to set this *)
+Arguments trans : simpl never.
+
+Section StrongSim.
+  Context {E F : Type} `{HE: Encode E} `{HF: Encode F} {X Y : Type}.
+  (*| The function defining strong simulations: [trans] plays must be answered
+    using [trans]. |*)
+  Program Definition ss (L : rel (label E) (label F)) :
+    mon (ctree E X -> ctree F Y -> Prop) :=
+    {| body R t u :=
+        forall l t', trans l t t' -> exists l' u', trans l' u u' /\ R t' u' /\ L l l'
+    |}.
+  Next Obligation.
+    unfold Proper, respectful, impl; intros.
+    edestruct H0 as (u' & l' & ?).
+    - apply H1. 
+    - exists u', l'; intuition.
+  Qed.
+
+  #[global] Instance weq_ss: Proper (weq ==> weq) ss.
+  Proof.
+    unfold Proper, respectful, weq; cbn; red; split; intros.
+    - apply H0 in H1 as (? & ? & ? & ? & ?).
+      exists x0, x1. split. apply H1. split. apply H2. apply H. apply H3.
+    - intros. apply H0 in H1 as (? & ? & ? & ? & ?).
+      exists x0, x1. split. apply H1. split. apply H2. apply H. apply H3.
+  Qed.
+
+  Definition ssim L := gfp (ss L).
+
+  #[global] Instance weq_ssim :
+    Proper (weq ==> weq) ssim.
+  Proof.
+    intros. split.
+    - intro. unfold ssim.
+      epose proof (gfp_weq (ss x) (ss y)). lapply H1.
+      + intro. red in H2. cbn in H2. rewrite <- H2. unfold ssim in H0. apply H0.
+      + now rewrite H.
+    - intro. unfold ssim.
+      epose proof (gfp_weq (ss x) (ss y)). lapply H1.
+      + intro. red in H2. cbn in H2. rewrite H2. apply H0.
+      + now rewrite H.
+  Qed.
+
+End StrongSim.
+
+(*| ss (simulation) notation |*)
+Notation sst L := (t (ss L)).
+Notation ssbt L := (bt (ss L)).
+Notation ssT L := (T (ss L)).
+Notation ssbT L := (bT (ss L)).
+
+Notation "t (≲ L ) u" := (ssim L t u) (at level 70): ctree_scope.
+Notation "t ≲ u" := (ssim eq t u) (at level 70): ctree_scope.
+Notation "t [≲ L ] u" := (ss L _ t u) (at level 79): ctree_scope.
+Notation "t [≲] u" := (ss eq _ t u) (at level 79): ctree_scope.
+Notation "t {≲ L } u" := (sst L _ t u) (at level 79): ctree_scope.
+Notation "t {≲} u" := (sst eq _ t u) (at level 79): ctree_scope.
+Notation "t {{≲ L }} u" := (ssbt L _ t u) (at level 79): ctree_scope.
+Notation "t {{≲}} u" := (ssbt eq _ t u) (at level 79): ctree_scope.
+
+Ltac fold_ssim :=
+  repeat
+    match goal with
+    | h: context[gfp (@ss ?E ?F ?HE ?HF ?X ?Y ?L)] |- _ => fold (@ssim E F HE HF X Y L) in h
+    | |- context[gfp (@ss ?E ?F ?HE ?HF ?X ?Y ?L)]      => fold (@ssim E F HE HF X Y L)
+    end.
+
+Ltac __coinduction_ssim R H :=
+  unfold ssim; apply_coinduction; fold_ssim; intros R H.
+
+#[global] Tactic Notation "__step_ssim" :=
+  match goal with
+  | |- context[@ssim ?E ?F ?C ?D ?X ?Y _ _ ?LR] =>
+      unfold ssim;
+      step;
+      fold (@ssim E F C D X Y _ _ L)
+  end.
+
+#[local] Tactic Notation "step" := __step_ssim || step.
+
+#[local] Tactic Notation "coinduction" simple_intropattern(R) simple_intropattern(H) :=
+  __coinduction_ssim R H || coinduction R H.
+
+#[global] Ltac __step_in_ssim H :=
+  match type of H with
+  | context[@ssim ?E ?F ?C ?D ?X ?Y ?LR] =>
+      unfold ssim in H;
+      step in H;
+      fold (@ssim E F C D X Y L) in H
+  end.
+
+#[local] Tactic Notation "step" "in" ident(H) :=
+  __step_in_ssim H || step in H.
+
+Import CTreeNotations.
+
+Section ssim_homogenous_theory.
+  Context {E: Type} `{HE: Encode E} {X: Type}
+          {L: relation (label E)}.
+
+  Notation ss := (@ss E E HE HE X X).
+  Notation ssim := (@ssim E E HE HE X X).
+  Notation sst L := (coinduction.t (ss L)).
+  Notation ssbt L := (coinduction.bt (ss L)).
+  Notation ssT L := (coinduction.T (ss L)).
+
+  (*| Various results on reflexivity and transitivity. |*)
+  Lemma refl_sst `{Reflexive _ L}: const eq <= (sst L).
+  Proof.    
+    apply leq_t; cbn; unfold impl; red; intros; subst; eauto.
+  Qed.
+
+  Lemma square_sst `{Transitive _ L}: square <= (sst L).
+  Proof.
+    apply Coinduction; cbn.
+    intros R x z [y xy yz] l x' xx'.
+    destruct (xy _ _ xx') as (l' & y' & yy' & ? & ?).
+    destruct (yz _ _ yy') as (l'' & z' & zz' & ? & ?).
+    exists l'', z'.
+    split.
+    assumption.
+    split.
+    apply (f_Tf (ss L)).
+    exists y'; eauto.
+    transitivity l'; auto.
+  Qed.
+
+  (*| Reflexivity |*)
+  #[global] Instance Reflexive_sst R `{Reflexive _ L}: Reflexive (sst L R).
+  Proof. apply build_reflexive; apply ft_t; apply (refl_sst). Qed.
+
+  Corollary Reflexive_ssim `{Reflexive _ L}: Reflexive (ssim L).
+  Proof. now apply Reflexive_sst. Qed.
+
+  #[global] Instance Reflexive_ssbt R `{Reflexive _ L}: Reflexive (ssbt L R).
+  Proof. apply build_reflexive; apply fbt_bt; apply refl_sst. Qed.
+
+  #[global] Instance Reflexive_ssT f R `{Reflexive _ L}: Reflexive (ssT L f R).
+  Proof. apply build_reflexive; apply fT_T; apply refl_sst. Qed.
+
+  (*| Transitivity |*)
+  #[global] Instance Transitive_sst R `{Transitive _ L}: Transitive (sst L R).
+  Proof. apply build_transitive; apply ft_t; apply (square_sst). Qed.
+
+  Corollary Transitive_ssim `{Transitive _ L}: Transitive (ssim L).
+  Proof. now apply Transitive_sst. Qed.
+
+  #[global] Instance Transitive_ssbt R `{Transitive _ L}: Transitive (ssbt L R).
+  Proof. apply build_transitive; apply fbt_bt; apply square_sst. Qed.
+
+  #[global] Instance Transitive_ssT f R `{Transitive _ L}: Transitive (ssT L f R).
+  Proof. apply build_transitive; apply fT_T; apply square_sst. Qed.
+
+  (*| PreOrder |*)
+  #[global] Instance PreOrder_sst R `{PreOrder _ L}: PreOrder (sst L R).
+  Proof. split; typeclasses eauto. Qed.
+
+  Corollary PreOrder_ssim `{PreOrder _ L}: PreOrder (ssim L).
+  Proof. split; typeclasses eauto. Qed.
+
+  #[global] Instance PreOrder_ssbt R `{PreOrder _ L}: PreOrder (ssbt L R).
+  Proof. split; typeclasses eauto. Qed.
+
+  #[global] Instance PreOrder_ssT f R `{PreOrder _ L}: PreOrder (ssT L f R).
+  Proof. split; typeclasses eauto. Qed.
+
+End ssim_homogenous_theory.
+
+(*| The LTS can not take a step [tau, vis, ret] |*)
+Definition is_stuck `{Encode E} {X} (t: ctree E X) := ( ~ exists l u, trans l t u).
+Arguments is_stuck /.
+
+Lemma stuck_is_stuck `{HE: Encode E} {X}:
+  @is_stuck E HE X stuck.
+Proof.
+  red; intros * abs; inv abs.
+  destruct H as (s' & TR).
+  ind_trans TR.
+  eapply IHTR; auto. 
+Qed.
+Global Hint Resolve stuck_is_stuck: ctree.
+
+(*| Parametric theory of [ss] with heterogenous relation on labels [L] |*)
+Section ssim_heterogenous_theory.
+  Context {E F: Type} `{HE: Encode E} `{HF: Encode F} {X Y: Type} {L: rel (label E) (label F)}.
+
+  Notation ss := (@ss E F HE HF X Y).
+  Notation ssim  := (@ssim E F HE HF X Y).
+  Notation sst L := (coinduction.t (ss L)).
+  Notation ssbt L := (coinduction.bt (ss L)).
+  Notation ssT L := (coinduction.T (ss L)).
+
+  (*| Strong simulation up-to [equ] is valid |*)
+  Lemma equ_clos_sst : equ_clos <= (sst L).
+  Proof.
+    apply Coinduction; cbn.
+    intros R x y [x' y' x'' y'' EQ' EQ''] l z x'z.
+    rewrite EQ' in x'z.
+    destruct (EQ'' _ _ x'z) as (l' & ? & ? & ? & ?).
+    exists l', x0.
+    split.
+    - rewrite <- Equu; auto.
+    - split; auto.
+      eapply (f_Tf (ss L)).
+      econstructor; auto; auto.
+  Qed.
+
+  #[global] Instance equ_clos_sst_goal {RR} :
+    Proper (equ eq ==> equ eq ==> flip impl) (sst L RR).
+  Proof.
+    cbn; intros ? ? eq1 ? ? eq2 H.
+    apply (ft_t equ_clos_sst); econstructor; [eauto | | symmetry; eauto]; assumption.
+  Qed.
+
+  #[global] Instance equ_clos_sst_ctx {RR} :
+    Proper (equ eq ==> equ eq ==> impl) (sst L RR).
+  Proof.
+    cbn; intros ? ? eq1 ? ? eq2 H.
+    apply (ft_t equ_clos_sst); econstructor; [symmetry; eauto | | eauto]; assumption.
+  Qed.
+
+  #[global] Instance equ_ssbt_closed_goal {r} :
+    Proper (equ eq ==> equ eq ==> flip impl) (ssbt L r).
+  Proof.
+    unfold Proper, respectful, impl, flip; intros.
+    apply (fbt_bt equ_clos_sst); econstructor; eauto.
+    now symmetry.
+  Qed.
+
+  #[global] Instance equ_ssbt_closed_ctx {r} :
+    Proper (equ eq ==> equ eq ==> impl) (ssbt L r).
+  Proof.
+    unfold Proper, respectful, impl, flip; intros.
+    now rewrite H, H0 in H1.
+  Qed.
+
+  #[global] Instance equ_clos_ssT_goal RR f :
+    Proper (equ eq ==> equ eq ==> flip impl) (ssT L f RR).
+  Proof.
+    unfold Proper, respectful, impl, flip; intros ? ? eq1 ? ? eq2 H.
+    apply (fT_T equ_clos_sst); econstructor; [eauto | | symmetry; eauto]; assumption.
+  Qed.
+
+  #[global] Instance equ_clos_ssT_ctx RR f :
+    Proper (equ eq ==> equ eq ==> impl) (ssT L f RR).
+  Proof.
+    unfold Proper, respectful, impl, flip; intros ? ? eq1 ? ? eq2 H.
+    apply (fT_T equ_clos_sst); econstructor; [symmetry; eauto | | eauto]; assumption.
+  Qed.
+
+  #[global] Instance equ_clos_ssim_goal :
+    Proper (equ eq ==> equ eq ==> flip impl) (ssim L).
+  Proof.
+    unfold Proper, respectful, impl, flip; intros ? ? eq1 ? ? eq2 H.
+    apply (ft_t equ_clos_sst); econstructor; [eauto | | symmetry; eauto]; assumption.
+  Qed.
+
+  #[global] Instance equ_clos_ssim_ctx :
+    Proper (equ eq ==> equ eq ==> impl) (ssim L).
+  Proof.
+    unfold Proper, respectful, impl, flip; intros ? ? eq1 ? ? eq2 H.
+    apply (ft_t equ_clos_sst); econstructor; [symmetry; eauto | | eauto]; assumption.
+  Qed.
+
+  #[global] Instance equ_ss_closed_goal {r} :
+    Proper (equ eq ==> equ eq ==> flip impl) (ss L r).
+  Proof.
+    unfold Proper, respectful, impl, flip, ss; cbn; intros t t' tt' u u' uu'; intros.
+    rewrite tt' in H0. apply H in H0 as (l' & ? & ? & ? & ?).
+    do 2 eexists; eauto. rewrite uu'. eauto.
+  Qed.
+
+  #[global] Instance equ_ss_closed_ctx {r} :
+    Proper (equ eq ==> equ eq ==> impl) (ss L r).
+  Proof.
+    unfold Proper, respectful, impl, flip, ss; cbn; intros t t' tt' u u' uu'; intros.
+    rewrite <- tt' in H0. apply H in H0 as (l' & ? & ? & ? & ?).
+    do 2 eexists; eauto. rewrite <- uu'. eauto.
+  Qed.
+    
+  (*| stuck ctrees can be simulated by anything. |*)
+  Lemma is_stuck_ss (R : rel _ _) (t : ctree E X) (t': ctree F Y):
+    is_stuck t -> ss L R t t'.
+  Proof.
+    repeat intro.
+    exfalso; apply H.
+    now (exists l, t'0).
+  Qed.
+
+  Lemma is_stuck_ssim (t: ctree E X) (t': ctree F Y):
+    is_stuck t -> ssim L t t'.
+  Proof.
+    intros; step.
+    cbn; intros.
+    exfalso; apply H.
+    now (exists l, t'0).
+  Qed.
+
+  Lemma stuck_ss (R : rel _ _) (t : ctree F Y) : ss L R stuck t.
+  Proof.
+    apply is_stuck_ss.
+    apply stuck_is_stuck.
+  Qed.
+
+  Lemma stuckD_ssim (t : ctree F Y) : ssim L stuck t.
+  Proof.
+    intros. step. apply stuck_ss.
+  Qed.
+
+End ssim_heterogenous_theory.
+
+
+(*|
+Up-to [bind] context simulations
+----------------------------------
+We have proved in the module [Equ] that up-to bind context is
+a valid enhancement to prove [equ].
+We now prove the same result, but for strong simulation.
+|*)
+
+Section ssim_heterogenous_bind.
+  Context {E F: Type} `{HE: Encode E} `{HF: Encode F} {X X' Y Y': Type}
+          (L : rel (label E) (label F)) (RR : rel X Y).
+
+  (* Mix of R0 for val and L for tau/obs. *)
+  Variant update_val_rel : label E -> label F -> Prop :=
+  | update_Val (v1 : X) (v2 : Y) : RR v1 v2 -> update_val_rel (val v1) (val v2)
+  | update_NonVal l1 l2 : ~is_val l1 -> ~is_val l2 -> L l1 l2 -> update_val_rel l1 l2.
+
+  Lemma update_val_rel_val : forall (v1 : X) (v2 : Y),
+    update_val_rel (val v1) (val v2) ->
+    RR v1 v2.
+  Proof.
+    intros. remember (val v1) as l1. remember (val v2) as l2.
+    destruct H.
+    - dependent destruction Heql1.
+      dependent destruction Heql2.
+      apply H. 
+    - subst. exfalso. now apply H.
+  Qed.
+
+  Lemma update_val_rel_val_l : forall (v1 : X) l2,
+    update_val_rel (val v1) l2 ->
+    exists v2 : Y, l2 = val v2 /\ RR v1 v2.
+  Proof.
+    intros. remember (val v1) as l1. destruct H.
+    - dependent destruction Heql1; eauto.
+    - subst. exfalso. apply H. constructor.
+  Qed.
+
+  Lemma update_val_rel_val_r : forall l1 (v2 : Y),
+    update_val_rel l1 (val v2) ->
+    exists v1 : X, l1 = val v1 /\ RR v1 v2.
+  Proof.
+    intros. remember (val v2) as l2. destruct H.
+    - dependent destruction Heql2. eauto.
+    - subst. exfalso. apply H0. constructor.
+  Qed.
+
+  Lemma update_val_rel_nonval_l : forall l1 l2,
+    update_val_rel l1 l2 ->
+    ~is_val l1 ->
+    ~is_val l2 /\ L l1 l2.
+  Proof.
+    intros. destruct H.
+    - exfalso. apply H0. constructor.
+    - auto.
+  Qed.
+
+  Lemma update_val_rel_nonval_r : forall l1 l2,
+    update_val_rel l1 l2 ->
+    ~is_val l2 ->
+    ~is_val l1 /\ L l1 l2.
+  Proof.
+    intros. destruct H.
+    - exfalso. apply H0. constructor.
+    - auto.
+  Qed.
+
+  Definition is_update_val_rel (L0 : rel (label E) (label F)) : Prop :=
+    forall l1 l2, wf_val X l1 -> wf_val Y l2 -> (L0 l1 l2 <-> update_val_rel l1 l2).
+
+  Theorem update_val_rel_correct : is_update_val_rel update_val_rel.
+  Proof.
+    red. reflexivity.
+  Qed.
+
+  (*| Specialization of [bind_ctx] to a function acting with [ssim] on the bound value,
+    and with the argument (pointwise) on the continuation. |*)
+  Program Definition bind_ctx_ssim L0 : mon (rel (ctree E X') (ctree F Y')) :=
+    {|body := fun R => @bind_ctx E F HE HF X Y X' Y' (ssim L0) (pointwise RR R) |}.
+  Next Obligation.
+    unfold Proper, respectful, impl; cbn; intros.
+    revert H0.
+    apply leq_bind_ctx. intros ?? H' ?? H''.
+    apply in_bind_ctx. apply H'. intros t t' HS. apply H, H'', HS.
+  Qed.
+
+  (*| The resulting enhancing function gives a valid up-to technique |*)
+  Lemma bind_ctx_ssim_t L0: 
+    is_update_val_rel L0 -> bind_ctx_ssim L0 <= (sst L).
+  Proof.
+    intro HL0. apply Coinduction.
+    intros R. apply (leq_bind_ctx _).
+    intros t1 t2 tt k1 k2 kk.
+    step in tt.
+    simpl; intros l u STEP;
+      apply trans_bind_inv in STEP as [(H & t' & STEP & EQ) | (v & STEPres & STEP)];
+      cbn in *.
+    apply tt in STEP as (u' & l' & STEP & EQ' & ?).
+    do 2 eexists. split.
+    apply trans_bind_l; eauto.
+    + intro Hl. destruct Hl.
+      apply HL0 in H0; etrans.
+      inv H0.
+      * now apply H. 
+      * now apply H2.
+    + split.
+      * apply (fT_T equ_clos_sst).
+        econstructor; [exact EQ | | reflexivity].
+        apply (fTf_Tf (ss L)).
+        apply in_bind_ctx; auto.
+        intros ? ? ?.
+        apply (b_T (ss L)).
+        red in kk; cbn; now apply kk.
+      * apply HL0 in H0; etrans.
+        destruct H0. exfalso. apply H. constructor. apply H2.
+    + apply tt in STEPres as (u' & ? & STEPres & EQ' & ?).
+      apply HL0 in H; etrans.
+      dependent destruction H. 2: { exfalso. apply H. constructor. }
+      pose proof (trans_val_inv STEPres) as EQ.
+      rewrite <- EQ in STEPres.
+      specialize (kk v v2 H).
+      apply kk in STEP as (u'' & ? & STEP & EQ'' & ?); cbn in *.
+      do 2 eexists; split.
+      eapply trans_bind_r; eauto.
+      split; auto.
+      eapply (id_T (ss L)); auto.
+  Qed.
+
+End ssim_heterogenous_bind.
+
+Theorem is_update_val_rel_eq `{HE: Encode E} {X} : @is_update_val_rel E E _ _ X X eq eq eq.
+Proof.
+  split; intro.
+  - subst. destruct l2.
+    + constructor; auto.
+      all: intro; inv H1.
+    + constructor; auto.
+      all: intro; inv H1.
+    + red in H. specialize (H X0 v eq_refl). subst.
+      constructor. reflexivity.
+  - inv H1; reflexivity.
+Qed.
+
+Theorem update_val_rel_eq `{HE: Encode E} {X} : forall l l', wf_val X l ->
+  @update_val_rel E E _ _ X X eq eq l l' <-> l = l'.
+Proof.
+  split; intro.
+  - destruct H0; now subst.
+  - subst. destruct l'.
+    3: { specialize (H X0 v eq_refl). subst. now left. }
+    all: constructor; auto; intro; inversion H0.
+Qed.
+
+Theorem update_val_rel_update_val_rel `{HE: Encode E} `{HF: Encode F} {X0 X1 Y0 Y1}
+    (L : rel (label E) (label F)) (R0 : rel X0 Y0) (R1 : rel X1 Y1) :
+  update_val_rel (update_val_rel L R0) R1 == update_val_rel L R1.
+Proof.
+  split; intro.
+  - destruct H.
+    + now constructor.
+    + destruct H1. { exfalso. now apply H. }
+      constructor; auto.
+  - destruct H.
+    + now constructor.
+    + constructor; auto.
+      constructor; auto.
+Qed.
+
+(*| Expliciting the reasoning rule provided by the up-to principles. |*)
+Lemma sst_clo_bind_gen `{HE: Encode E} `{HF: Encode F} {X Y X' Y': Type} {L : rel (label E) (label F)}
+      (R0 : rel X Y) L0
+      (t1 : ctree E X) (t2: ctree F Y)
+      (HL0 : is_update_val_rel L R0 L0)
+      (k1 : X -> ctree E X') (k2 : Y -> ctree F Y') RR:
+  t1 (≲L0) t2 ->
+  (forall x y, R0 x y -> (sst L RR) (k1 x) (k2 y)) ->
+  sst L RR (t1 >>= k1) (t2 >>= k2).
+Proof.
+  intros ? ?.
+  apply (ft_t (@bind_ctx_ssim_t E F HE HF X X' Y Y' L R0 L0 HL0)).
+  apply in_bind_ctx; eauto.
+Qed.
+
+Lemma sst_clo_bind `{HE: Encode E} `{HF: Encode F} {X Y X' Y': Type} {L : rel (label E) (label F)}
+      (R0 : rel X Y)
+      (t1 : ctree E X) (t2: ctree F Y)
+      (k1 : X -> ctree E X') (k2 : Y -> ctree F Y') RR:
+  t1 (≲update_val_rel L R0) t2 ->
+  (forall x y, R0 x y -> (sst L RR) (k1 x) (k2 y)) ->
+  sst L RR (t1 >>= k1) (t2 >>= k2).
+Proof.
+  intros ? ?.
+  eapply sst_clo_bind_gen; eauto.
+  apply update_val_rel_correct.
+Qed.
+
+Lemma sst_clo_bind_eq `{HE: Encode E} `{HF: Encode F} {X X': Type}
+      (t1 : ctree E X) (t2: ctree E X)
+      (k1 : X -> ctree E X') (k2 : X -> ctree E X') RR:
+  t1 ≲ t2 ->
+  (forall x, sst eq RR (k1 x) (k2 x)) ->
+  sst eq RR (t1 >>= k1) (t2 >>= k2).
+Proof.
+  intros ? ?.
+  eapply sst_clo_bind_gen.
+  - apply is_update_val_rel_eq.
+  - assumption.
+  - intros. now subst.
+Qed.
+
+Lemma ssbt_clo_bind_gen `{HE: Encode E} `{HF: Encode F} {X Y X' Y': Type}
+  {L : rel (label E) (label F)}
+      (R0 : rel X Y) L0
+      (t1 : ctree E X) (t2: ctree F Y)
+      (HL0 : is_update_val_rel L R0 L0)
+      (k1 : X -> ctree E X') (k2 : Y -> ctree F Y') RR:
+  t1 (≲L0) t2 ->
+  (forall x y, R0 x y -> (ssbt L RR) (k1 x) (k2 y)) ->
+  ssbt L RR (t1 >>= k1) (t2 >>= k2).
+Proof.
+  intros ? ?.
+  apply (fbt_bt (@bind_ctx_ssim_t E F HE HF X X' Y Y' L R0 L0 HL0)).
+  apply in_bind_ctx; eauto.
+Qed.
+
+Lemma ssbt_clo_bind `{HE: Encode E} `{HF: Encode F} {X Y X' Y': Type}
+  {L : rel (label E) (label F)}
+      (R0 : rel X Y)
+      (t1 : ctree E X) (t2: ctree F Y)
+      (k1 : X -> ctree E X') (k2 : Y -> ctree F Y') RR:
+  t1 (≲update_val_rel L R0) t2 ->
+  (forall x y, R0 x y -> (ssbt L RR) (k1 x) (k2 y)) ->
+  ssbt L RR (t1 >>= k1) (t2 >>= k2).
+Proof.
+  intros ? ?.
+  eapply ssbt_clo_bind_gen; eauto.
+  apply update_val_rel_correct.
+Qed.
+
+Lemma ssbt_clo_bind_eq `{HE: Encode E} `{HF: Encode F} {X X': Type}
+      (t1 : ctree E X) (t2: ctree E X)
+      (k1 : X -> ctree E X') (k2 : X -> ctree E X') RR:
+  t1 ≲ t2 ->
+  (forall x, ssbt eq RR (k1 x) (k2 x)) ->
+  ssbt eq RR (t1 >>= k1) (t2 >>= k2).
+Proof.
+  intros ? ?.
+  eapply ssbt_clo_bind_gen.
+  - apply is_update_val_rel_eq.
+  - assumption.
+  - intros. now subst.
+Qed.
+
+(*| Specializing the congruence principle for [≲] |*)
+Lemma ssim_clo_bind_gen `{HE: Encode E} `{HF: Encode F} {X Y X' Y': Type}
+  {L : rel (label E) (label F)}
+      (R0 : rel X Y) L0
+      (HL0 : is_update_val_rel L R0 L0)
+      (t1 : ctree E X) (t2: ctree F Y)
+      (k1 : X -> ctree E X') (k2 : Y -> ctree F Y'):
+  ssim L0 t1 t2 ->
+  (forall x y, R0 x y -> ssim L (k1 x) (k2 y)) ->
+  ssim L (t1 >>= k1) (t2 >>= k2).
+Proof.
+  intros. eapply sst_clo_bind_gen; eauto.
+Qed.
+
+Lemma ssim_clo_bind `{HE: Encode E} `{HF: Encode F} {X Y X' Y': Type}
+  {L : rel (label E) (label F)}
+  (R0 : rel X Y)
+  (t1 : ctree E X) (t2: ctree F Y)
+  (k1 : X -> ctree E X') (k2 : Y -> ctree F Y'):
+  t1 (≲update_val_rel L R0) t2 ->
+  (forall x y, R0 x y -> k1 x (≲L) k2 y) ->
+  t1 >>= k1 (≲L) t2 >>= k2.
+Proof.
+  intros. eapply sst_clo_bind; eauto.
+Qed.
+
+Lemma ssim_clo_bind_eq `{HE: Encode E} `{HF: Encode F} {X X': Type}
+      (t1 : ctree E X) (t2: ctree E X)
+      (k1 : X -> ctree E X') (k2 : X -> ctree E X'):
+  t1 ≲ t2 ->
+  (forall x, k1 x ≲ k2 x) ->
+  t1 >>= k1 ≲ t2 >>= k2.
+Proof.
+  intros. apply sst_clo_bind_eq; auto.
+Qed.
+
+Tactic Notation "__upto_bind_ssim" uconstr(R0) :=
+  match goal with
+    |- @ssim ?E ?F ?C ?D ?X ?Y ?L (Ctree.bind (X := ?T) _ _) (Ctree.bind (X := ?T') _ _) =>
+      apply (ssim_clo_bind_gen R0 (update_val_rel L R0) (update_val_rel_correct L R0))
+  | |- body (t (@ss ?E ?F ?C ?D ?X ?Y ?L)) ?R (Ctree.bind (X := ?T) _ _) (Ctree.bind (X := ?T') _ _) =>
+      apply (ft_t (@bind_ctx_ssim_t E F C D T X T' Y L R0
+        (update_val_rel L R0) (update_val_rel_correct L R0))), in_bind_ctx
+  | |- body (bt (@ss ?E ?F ?C ?D ?X ?Y ?L)) ?R (Ctree.bind (X := ?T) _ _) (Ctree.bind (X := ?T') _ _) =>
+      apply (fbt_bt (@bind_ctx_ssim_t E F C D T X T' Y L R0
+        (update_val_rel L R0) (update_val_rel_correct L R0))), in_bind_ctx
+  end.
+
+Tactic Notation "__upto_bind_eq_ssim" uconstr(R0) :=
+  match goal with
+  | |- @ssim ?E ?F ?C ?D ?X ?Y ?L (Ctree.bind (X := ?T) _ _) (Ctree.bind (X := ?T') _ _) =>
+      __upto_bind_ssim R0; [reflexivity | intros ?]
+  | _ => __upto_bind_ssim R0; [reflexivity | intros ? ? ?EQl]
+  end.
+
+Ltac __play_ssim := step; cbn; intros ? ? ?TR.
+
+Ltac __play_ssim_in H :=
+  step in H;
+  cbn in H; edestruct H as (? & ? & ?TR & ?EQ & ?HL);
+  clear H; [etrans |].
+
+Ltac __eplay_ssim :=
+  match goal with
+  | h : @ssim ?E ?F ?C ?D ?X ?Y ?L _ _ |- _ =>
+      __play_ssim_in h
+  end.
+
+#[local] Tactic Notation "play" := __play_ssim.
+#[local] Tactic Notation "play" "in" ident(H) := __play_ssim_in H.
+#[local] Tactic Notation "eplay" := __eplay_ssim.
+
+Section Proof_Rules.
+  Context `{HE: Encode E} `{HF: Encode F} {X : Type}.
+
+  Lemma step_ss_ret_gen {Y} (x : X) (y : Y) (R L : rel _ _) :
+    R stuck stuck ->
+    (Proper (equ eq ==> equ eq ==> impl) R) ->
+    L (val x) (val y) ->
+    ss L R (Ret x : ctree E X) (Ret y : ctree F Y).
+  Proof.
+    intros Rstuck PROP Lval.
+    cbn; intros ? ? TR.
+    apply trans_ret_inv in TR as (? & ->).
+    exists (val y), stuck; split; etrans.
+    rewrite H; auto.
+  Qed.
+
+  Lemma step_ss_ret {Y} (x : X) (y : Y) (R L : rel _ _) :
+    L (val x) (val y) ->
+    ssbt L R (Ret x : ctree E X) (Ret y : ctree F Y).
+  Proof.
+    intros.
+    apply step_ss_ret_gen.
+    - step. intros.
+      apply is_stuck_ss.
+      eapply stuck_is_stuck. 
+    - typeclasses eauto.
+    - apply H.
+  Qed.
+
+  Lemma ssim_ret {Y} (x : X) (y : Y) (L : rel _ _) :
+    L (val x) (val y) ->
+    ssim L (Ret x : ctree E X) (Ret y : ctree F Y).
+  Proof.
+    intros. step. now apply step_ss_ret.
+  Qed.
+
+(*|
+ The vis nodes are deterministic from the perspective of the labeled
+ transition system, stepping is hence symmetric and we can just recover
+ the itree-style rule.
+|*)
+  Lemma step_ss_vis_gen {Y} (e : E) (f: F)
+        (k : encode e -> ctree E X) (k' : encode f -> ctree F Y) (R L: rel _ _) :
+    (Proper (equ eq ==> equ eq ==> impl) R) ->
+    (forall x, exists y, R (k x) (k' y) /\ L (obs e x) (obs f y)) ->
+    ss L R (Vis e k) (Vis f k').
+  Proof.
+    intros.
+    cbn; intros ? ? TR.
+    apply trans_vis_inv in TR as (x & ? & ->).
+    destruct (H0 x) as (x' & RR & LL);
+      cbn; eexists; eexists; intuition.
+    - rewrite H1; eauto.
+    - assumption.
+  Qed.
+
+  Lemma step_ss_vis {Y} (e : E) (f: F)
+        (k : encode e -> ctree E X) (k': encode f  -> ctree F Y) (R L : rel _ _) :
+    (forall x, exists y, sst L R (k x) (k' y) /\ L (obs e x) (obs f y)) ->
+    ssbt L R (Vis e k) (Vis f k').
+  Proof.
+    intros * EQ.
+    apply step_ss_vis_gen; auto.
+    typeclasses eauto.
+  Qed.
+
+  Lemma ssim_vis {Y} (e : E) (f: F)
+        (k : encode e -> ctree E X) (k' : encode f -> ctree F Y) (L : rel _ _) :
+    (forall x, exists y, ssim L (k x) (k' y) /\ L (obs e x) (obs f y)) ->
+    ssim L (Vis e k) (Vis f k').
+  Proof.
+    intros. step. now apply step_ss_vis.
+  Qed.
+
+  (*| Same goes for visible tau nodes. |*)
+  Lemma step_ss_step_gen {Y}
+        (t : ctree E X) (t': ctree F Y) (R L: rel _ _):
+    (Proper (equ eq ==> equ eq ==> impl) R) ->
+    L tau tau ->
+    (R t t') ->
+    ss L R (step t) (step t').
+  Proof.
+    intros PR ? EQs.
+    intros ? ? TR.
+    apply trans_br_inv in TR as ([] & ? & ->).
+    all: exists tau, t'; split; [etrans|]; split; [rewrite H0|]; auto.
+  Qed.
+
+  Lemma step_ss_step {Y} (t: ctree E X) (t': ctree F Y) (R L : rel _ _) :
+    (sst L R t t') ->
+    L tau tau ->
+    ssbt L R (step t) (step t').
+  Proof.
+    intros. apply step_ss_step_gen; auto.
+    typeclasses eauto.
+  Qed.
+
+  (*|
+    When matching visible brs one against another, in general we need to explain how
+    we map the branches from the left to the branches to the right.
+    A useful special case is the one where the arity coincide and we simply use the identity
+    in both directions. We can in this case have [n] rather than [2n] obligations.
+    |*)
+  Lemma step_ss_br_gen {Y n m} (k : fin' n -> ctree E X) (k' : fin' m -> ctree F Y)
+    (R L: rel _ _) :
+    (Proper (equ eq ==> equ eq ==> impl) R) ->
+    (forall x, exists y, R (k x) (k' y)) ->
+    L tau tau ->
+    ss L R (Br n k) (Br m k').
+  Proof.
+    intros PROP EQs ? ? ? TR.
+    apply trans_br_inv in TR as (? & ? & ->).
+    destruct (EQs x) as [y HR].
+    cbn; do 2 eexists; split; [etrans | split; [rewrite H0; eauto|assumption]].
+  Qed.
+
+  Lemma step_ss_br {Y n m} (k : fin' n -> ctree E X) (k' : fin' m -> ctree F Y)
+    (R L: rel _ _) :
+    (forall x, exists y, sst L R (k x) (k' y)) ->
+    L tau tau ->
+    ssbt L R (Br n k) (Br m k').
+  Proof.
+    intros.
+    apply step_ss_br_gen; auto.
+    typeclasses eauto.
+  Qed.
+
+  Lemma ssim_br {Y n m} (k : fin' n -> ctree E X) (k' : fin' m -> ctree F Y) (L: rel _ _) :
+    (forall x, exists y, ssim L (k x) (k' y)) ->
+    L tau tau ->
+    ssim L (Br n k) (Br m k').
+  Proof.
+    intros. step. now apply step_ss_br.
+  Qed.
+
+  Lemma step_ss_br_id_gen {Y n} (k: fin' n -> ctree E X) (k': fin' n -> ctree F Y)
+    (R L : rel _ _) :
+    (Proper (equ eq ==> equ eq ==> impl) R) ->
+    (forall x, exists y, R (k x) (k' y)) ->
+    L tau tau ->
+    ss L R (Br n k) (Br n k').
+  Proof.
+    intros; apply step_ss_br_gen; eauto.
+  Qed.
+
+  Lemma step_ss_br_id {Y n} (k: fin' n -> ctree E X) (k': fin' n -> ctree F Y) (R L : rel _ _) :
+    (forall x, exists y, sst L R (k x) (k' y)) ->
+    L tau tau ->
+    ssbt L R (Br n k) (Br n k').
+  Proof.
+    intros.
+    apply step_ss_br_id_gen; eauto.
+    typeclasses eauto.
+  Qed.
+
+  Lemma ssim_br_id {Y n} (k: fin' n -> ctree E X) (k': fin' n -> ctree F Y) (L : rel _ _) :
+    (forall x, exists y, ssim L (k x) (k' y)) ->
+    L tau tau ->
+    ssim L (Br n k) (Br n k').
+  Proof.
+    intros. step. now apply step_ss_br_id.
+  Qed.
+
+  Lemma ssim_step {Y} (t: ctree E X) (t': ctree F Y) (L : rel _ _) :
+    ssim L t t' ->
+    L tau tau ->
+    ssim L (step t) (step t').
+  Proof.
+    intros. apply ssim_br_id; eauto.
+  Qed.
+
+  (*|
+    For invisible nodes, the situation is different: we may kill them, but that execution
+    cannot act as going under the guard.
+    |*)
+  Lemma step_ss_guard_gen {Y} (t: ctree E X) (t': ctree F Y) (R L: rel _ _):
+    ss L R t t' ->
+    ss L R (Guard t) (Guard t').
+  Proof.
+    intros EQ.
+    intros ? ? TR.
+    apply trans_guard_inv in TR.
+    apply EQ in TR as (? & ? & ? & ? & ?); subst.
+    do 2 eexists; split; [etrans | split; trivial].
+  Qed.
+
+  Lemma step_ss_guard {Y} (t: ctree E X) (t': ctree F Y) (R L: rel _ _):
+    ssbt L R t t' ->
+    ssbt L R (Guard t) (Guard t').
+  Proof.
+    apply step_ss_guard_gen.
+  Qed.
+
+  (*| Inversion principles |*)
+  Lemma ssim_ret_inv {Y} {L: rel (label E) (label F)} r1 r2:
+    ssim L (Ret r1 : ctree E X) (Ret r2 : ctree F Y) ->
+    L (val r1) (val r2).
+  Proof.
+    intro.
+    eplay.
+    now trans in TR. 
+  Qed.
+
+  Lemma ssbt_vis_inv {Y} {L: rel (label E) (label F)}
+    (e: E) (f : F) (k1 : encode e -> ctree E X) (k2 : encode f -> ctree F Y) x R:
+    ssbt L R (Vis e k1) (Vis f k2) ->
+    (exists y, L (obs e x) (obs f y))  /\ (forall x, exists y, sst L R (k1 x) (k2 y)).
+  Proof.
+    intros.
+    split; intros; edestruct H as (? & ? & ? & ? & ?);
+      etrans; trans in H0; eexists; eauto.
+    rewrite <- Eqt; apply H1.
+  Qed.
+
+  Lemma ssim_vis_inv {Y} {L: rel (label E) (label F)}
+        (e: E) (f : F) (k1 : encode e -> ctree E X) (k2 : encode f -> ctree F Y) x:
+    ssim L (Vis e k1) (Vis f k2) ->
+    (exists y, L (obs e x) (obs f y)) /\ (forall x, exists y, ssim L (k1 x) (k2 y)).
+  Proof.
+    intros.
+    split.
+    - eplay.
+      trans in TR.
+      exists x2; eauto.
+    - intros y.
+      step in H.
+      cbn in H.
+      edestruct H as (l' & u' & TR & IN & HL).
+      apply trans_vis with (x := y).
+      trans in TR.
+      exists x0.
+      rewrite <- Eqt.
+      apply IN.
+  Qed.
+
+  Lemma ssim_br_inv {Y n m} {L: rel (label E) (label F)}
+    (k1 : fin' n -> ctree E X) (k2 : fin' m -> ctree F Y) :
+    ssim L (Br n k1) (Br m k2) ->
+    (forall i1, exists i2, ssim L (k1 i1) (k2 i2)).
+  Proof.
+    intros EQ i1.
+    eplay.
+    trans in TR.
+    rewrite Eqt in EQ0.
+    (exists n0); eauto.
+  Qed.
+
+End Proof_Rules.
