theories/CTree/Trans.v
@@ -1,0 +1,621 @@
+(*|
+==========================================
+Transition relations over ctrees
+==========================================
+
+Trees represent the dynamics of non-deterministic procesess.
+In order to capture their behavioral equivalence, we follow the
+process-algebra tradition and define bisimulation atop of labelled
+transition systems.
+
+A node is said to be _observable_ if it is a visible event, a return
+node, or an internal br tagged as visible.
+The first transition relation we introduce is [trans]: a tree can
+finitely descend through unobservable brs until it reaches an
+observable node. At this point, it steps following the simple rules:
+- [Ret v] steps to a silently blocked state by emitting a value
+label of [v]
+- [Vis e k] can step to any [k x] by emitting an event label tagged
+with both [e] and [x]
+- [BrS k] can step to any [k x] by emitting a tau label
+
+This transition system will define a notion of strong bisimulation
+in the process algebra tradition.
+It also leads to a weak bisimulation by defining [wtrans] as a
+sequence of tau steps, and allowing a challenge to be answered by
+[wtrans . trans . wtrans].
+Once [trans] is defined over our structure, we can reuse the constructions
+used by Pous in [Coinduction All the Way Up] to build these weak relations
+-- with the exception that we need to work in Kleene Algebras w.r.t. to model
+closed under [equ] rather than [eq].
+
+.. coq:: none
+|*)
+
+From Coq Require Import
+  Basics
+  Datatypes
+  Fin.
+
+From Coinduction Require Import
+     coinduction rel tactics.
+
+From CTree Require Import
+  CTree.Core
+  CTree.Equ.
+
+Import Ctree.
+Import CTreeNotations.
+Local Open Scope ctree_scope.
+
+Generalizable All Variables.
+Set Implicit Arguments.
+Set Primitive Projections.
+
+Section Trans.
+  Context {E : Type} `{HE: Encode E} {X : Type}.
+
+(*|
+The domain of labels of the LTS.
+Note that it could be typed more strongly: [val] labels can only
+be of type [R]. However typing it statically makes lemmas about
+[bind] particularly awkward to state, so this seems to be the
+least annoying solution.
+|*)
+  Variant label : Type :=
+    | tau
+    | obs (e : E) (v : encode e)
+    | val {X : Type} (v : X).
+
+(*|
+The transition relation over [ctree]s.
+It can either:
+- recursively crawl through invisible [br] node;
+- stop at a successor of a visible [br] node, labelling the transition [tau];
+- stop at a successor of a [Vis] node, labelling the transition by the event and branch taken;
+- stop at a sink (implemented as a [spin] node that has no successor.
+|*)
+  Inductive trans_ : label -> relation (ctree' E X) :=
+
+  | Stepguard l t u:
+    trans_ l (observe t) u ->
+    trans_ l (GuardF t) u
+
+  | Steptau {n} (x : fin' n) k t :
+    k x ≅ t ->
+    trans_ tau (BrF n k) (observe t)
+
+  | Stepobs (e : E) k (x: encode e) t :
+    k x ≅ t ->
+    trans_ (obs x) (VisF e k) (observe t)
+
+  | Stepval t r :
+    stuck ≅ t ->
+    trans_ (val r) (RetF r) (observe t).
+  Hint Constructors trans_ : core.
+
+  Definition trans l : relation (ctree E X) :=
+    fun u v => trans_ l (observe u) (observe v).
+
+  #[local] Instance trans_equ_aux1 l t :
+    Proper (going (equ eq) ==> flip impl) (trans_ l t).
+  Proof.
+    intros u u' equ; intros TR.
+    inv equ; rename H into equ.
+    step in equ.
+    revert u equ.
+    dependent induction TR; intros.
+    + econstructor.
+      now apply IHTR.
+    + inv equ; cbn in H1; rewrite <- H1.
+      * rewrite H0; now apply Steptau with x. 
+      * change (VisF e k1) with (observe (Vis e k1)).
+        apply (Steptau x).
+        rewrite H.
+        rewrite (ctree_eta t); rewrite <- H0. 
+        step; constructor; intros; symmetry; auto.
+      * change (BrF n k) with (observe (Br n k)).
+        change (GuardF t1) with (observe (Guard t1)).
+        apply (Steptau x).
+        rewrite H.
+        rewrite (ctree_eta t), <- H0.
+        step; constructor; intros; symmetry; auto.
+      * change (BrF n k) with (observe (Br n k)).
+        change (BrF n0 k1) with (observe (Br n0 k1)).
+        apply (Steptau x). 
+        rewrite H.
+        rewrite (ctree_eta t), <- H0.
+        step; constructor; intros; symmetry; auto.
+    + change u with (observe (go u)).
+      econstructor.
+      rewrite H; symmetry; step; auto.
+    + change u with (observe (go u)).
+      cbn in equ.
+      econstructor.
+      rewrite H.
+      symmetry.
+      step; cbn; apply equ.
+  Qed.
+
+  #[local] Instance trans_equ_aux2 l :
+    Proper (going (equ eq) ==> going (equ eq) ==> impl) (trans_ l).
+  Proof.
+    intros t t' eqt u u' equ TR.
+    rewrite <- equ; clear u' equ.
+    inv eqt; rename H into eqt.
+    revert t' eqt.
+    dependent induction TR; intros; auto.
+    + step in eqt; cbn in eqt; dependent induction eqt.
+      apply Stepguard.
+      apply IHTR.
+      rewrite H; reflexivity.
+    + step in eqt; cbn in eqt; dependent induction eqt.
+      apply Steptau with x.
+      now rewrite <- H0.
+    + step in eqt; cbn in eqt; dependent induction eqt.
+      econstructor.
+      rewrite <- H.
+      now symmetry.
+    + step in eqt; cbn in eqt; dependent induction eqt.
+      now econstructor.
+  Qed.
+
+  #[global] Instance trans_equ_ l :
+    Proper (going (equ eq) ==> going (equ eq) ==> iff) (trans_ l).
+  Proof.
+    intros ? ? eqt ? ? equ; split; intros TR.
+    - eapply trans_equ_aux2; eauto.
+    - symmetry in equ; symmetry in eqt; eapply trans_equ_aux2; eauto.
+  Qed.
+
+  #[global] Instance trans_equ l :
+    Proper (equ eq ==> equ eq ==> iff) (trans l).
+  Proof.
+    intros ? ? eqt ? ? equ; unfold trans.
+    rewrite eqt, equ; reflexivity.
+  Qed.
+
+End Trans.
+
+Ltac ind_trans H :=
+  unfold trans, trans in H; cbn in H;
+  dependent induction H.
+
+Section Trans.
+  Context {E : Type} `{HE: Encode E} {X : Type}. 
+
+  (*| Backward reasoning for [trans] |*)
+  Lemma trans_ret : forall (x : X),
+      trans (val x) (Ret x) stuck.
+  Proof. intros; now constructor. Qed.
+
+  Lemma trans_vis : forall (e : E) (x: encode e) (k : encode e -> ctree E X),
+      trans (obs e x) (Vis e k) (k x).
+  Proof. intros; now constructor. Qed.
+
+  Lemma trans_guard : forall l (t u: ctree E X),
+      trans l t u ->
+      trans l (Guard t) u.
+  Proof.
+    intros * TR.
+    apply Stepguard.
+    apply TR.
+  Qed.
+
+  Lemma trans_br : forall n (k : _ -> ctree E X) t x,
+      k x ≅ t ->
+      trans tau (Br n k) t.
+  Proof.
+    intros.
+    apply Steptau with x; apply H. 
+  Qed.
+
+  Lemma trans_step : forall (t: ctree E X),
+      trans tau (step t) t.
+  Proof.
+    intros.
+    apply Steptau; [exact Fin.F1 | reflexivity].
+  Qed.
+
+  Lemma trans_br2_l : forall (t u: ctree E X),
+      trans tau (br2 t u) t.
+  Proof.
+    intros.
+    unfold br2.
+    apply trans_br with Fin.F1.
+    reflexivity.
+  Qed.
+
+  Lemma trans_br2_r: forall (t u: ctree E X),
+      trans tau (br2 t u) u.
+  Proof.
+    intros.
+    unfold br2.
+    eapply trans_br with (Fin.FS Fin.F1).
+    reflexivity.
+  Qed.
+
+  (*| Forward reasoning for [trans] |*)
+  Lemma trans_ret_inv : forall x l (t : ctree E X),
+      trans l (Ret x) t ->
+       t ≅ stuck /\ l = val x.
+  Proof.
+    intros * TR; inv TR; intuition.
+    observe_equ H1.
+    symmetry.
+    now rewrite <- Eqt.
+  Qed.
+
+  Lemma trans_vis_inv : forall (e : E) (k: encode e -> _) l (u : ctree E X),
+      trans l (Vis e k) u ->
+      exists x, u ≅ k x /\ l = obs e x.
+  Proof.
+    intros * TR.
+    ind_trans TR.
+    observe_equ x.
+    exists x0; split.
+    - rewrite H; now symmetry.
+    - reflexivity.
+  Qed.
+
+  Lemma trans_guard_inv : forall l (t u : ctree E X),
+      trans l (Guard t) u ->
+      trans l t u.
+  Proof.
+    intros * TR.
+    unfold trans in *.
+    cbn in TR |- *.
+    match goal with
+    | h: trans_ _ ?x ?y |- _ =>
+        remember x as ox; remember y as oy
+    end.
+    clear Heqoy u.
+    induction TR; intros; dependent destruction Heqox;
+      eauto.
+  Qed.
+
+  Lemma trans_br_inv : forall n k l (t' : ctree E X),
+      trans l (Br n k) t' ->
+      exists x, t' ≅ k x /\ l = tau.
+  Proof.
+    intros * TR.
+    cbn in *; red in TR; cbn in TR.
+    dependent induction TR.
+    eexists; split; auto.
+    rewrite H, ctree_eta, (ctree_eta t), x; reflexivity.
+  Qed.
+
+  Lemma trans_step_inv: forall l (t t': ctree E X),
+      trans l (step t) t' ->
+      t' ≅ t /\ l = tau.
+  Proof.
+    intros * TR; apply trans_br_inv in TR as (_ & ? & ?); auto.
+  Qed.
+
+  Lemma trans_br2_inv : forall l (t t' u : ctree E X),
+      trans l (br2 t u) t' ->
+      (l = tau /\ (t' ≅ t \/ t' ≅ u)).
+  Proof.
+    intros * TR; apply trans_br_inv in TR as (? & TR & ->); split; auto.
+    destruct x; auto.
+  Qed.
+
+  Lemma trans_br3_inv : forall l (t t' u v: ctree E X),
+      trans l (br3 t u v) t' ->
+      (l = tau /\ (t' ≅ t \/ t' ≅ u \/ t' ≅ v)).
+  Proof.
+    intros * TR.
+    apply trans_br_inv in TR as (? & TR & ->); split; [reflexivity|].
+    dependent destruction x; [|dependent destruction x].
+    - now left.
+    - now right; left.
+    - now right; right.
+  Qed.
+  
+  (*| Inversion rules for [trans] based on the value of the label |*)
+  Lemma trans__val_inv {Y} : 
+    forall (T U : ctree' E X) (x : Y),
+      trans_ (val x) T U ->
+      stuck ≅ go U.
+  Proof.
+    intros * TR.
+    remember (val x) as ox.
+    rewrite ctree_eta; induction TR; intros; auto; try now inv Heqox.
+    rewrite H.
+    reflexivity.
+  Qed.
+
+  Lemma trans_val_inv {Y} :
+    forall (t u : ctree E X) (x : Y),
+      trans (val x) t u ->
+      stuck ≅ u.
+  Proof.
+    intros * TR. cbn in TR. red in TR.
+    apply trans__val_inv in TR. rewrite ctree_eta.
+    rewrite (ctree_eta u), TR.
+    reflexivity.
+  Qed.
+
+  Lemma trans_stuck: forall l (t: ctree E X),
+      ~ trans l stuck t.
+  Proof.
+    intros * Hcontra.
+    unfold trans in Hcontra.
+    dependent induction Hcontra.
+    eapply IHHcontra; reflexivity.
+  Qed.
+  Hint Resolve trans_stuck: trans.
+
+End Trans.
+
+Arguments label E {_}.
+
+(*| Forward and backward rules for [trans] w.r.t. [bind] |*)
+Variant is_val `{Encode E}: label E -> Prop :=
+  | Is_val : forall X (x : X), is_val (val x).
+
+Lemma trans_bind_inv_aux {X Y} `{HE: Encode E} (l: label E)  T U :
+  trans_ l T U ->
+  forall (t : ctree E X) (k : X -> ctree E Y) (u : ctree E Y),
+    go T ≅ t >>= k ->
+    go U ≅ u ->
+    (~ (is_val l) /\ exists t', trans l t t' /\ u ≅ t' >>= k) \/
+      (exists (x : X), trans (val x) t stuck /\ trans l (k x) u).
+Proof.
+  intros TR; induction TR; intros.
+  - rewrite unfold_bind in H; setoid_rewrite (ctree_eta t0).
+    desobs t0.
+    + right.
+      exists x; split.
+      constructor.
+      reflexivity.
+      rewrite <- H.
+      apply Stepguard; auto.
+      rewrite <- H0; auto.
+    + step in H; cbn in H; inversion H.
+    + step in H; cbn in H; dependent destruction H.
+      specialize (IHTR t1 k u0).
+      destruct IHTR as [(? & ? & ? & ?) | (? & ? & ?)]; auto.
+      rewrite <- ctree_eta, H; reflexivity.
+      left; split; eauto.
+      exists x; split; auto.
+      apply Stepguard; auto.
+      right.
+      exists x; split; auto.
+      apply Stepguard; auto.
+    + step in H; inversion H.
+  - rewrite unfold_bind in H0; setoid_rewrite (ctree_eta t0).
+    desobs t0.
+    + right.
+      exists x0; split.
+      constructor.
+      reflexivity.
+      rewrite <- H0.
+      apply (Steptau x); auto.
+      rewrite H, <- H1, ctree_eta; auto.
+    + step in H0; cbn in H0; dependent induction H0.
+      left; split; [intros abs; inv abs |].
+      exists (k1 x); split.
+      econstructor; reflexivity.
+      rewrite <- H1, <- ctree_eta, <- H.
+      apply H0.
+    + step in H0; inversion H0.
+    + step in H0; inversion H0.
+  - rewrite unfold_bind in H0; setoid_rewrite (ctree_eta t0).
+    desobs t0.
+    + right.
+      exists x0; split.
+      constructor.
+      reflexivity.
+      rewrite <- H0.
+      constructor.
+      rewrite H, <- H1, ctree_eta; auto.
+    + step in H0; inversion H0.
+    + step in H0; cbn in H0; inversion H0. 
+    + step in H0; cbn in H0; dependent destruction H0.
+      left; split; [intros abs; inv abs |].
+      exists (k1 x); split.
+      econstructor; reflexivity.
+      rewrite <- H1, <- ctree_eta, <- H.
+      apply H0.
+  - rewrite unfold_bind in H0.
+    setoid_rewrite (ctree_eta t0).
+    desobs t0.
+    + right.
+      exists x; split.
+      constructor.
+      reflexivity.
+      rewrite <- H1, <- H0, <- ctree_eta.
+      now constructor.
+    + step in H0; inversion H0.
+    + step in H0; inversion H0.
+    + step in H0; inversion H0.
+Qed.
+
+Lemma trans_bind_inv {X Y} `{HE: Encode E} (t : ctree E X)
+  (k : X -> ctree E Y) (u : ctree E Y) (l: label E) :
+  trans l (t >>= k) u ->
+  (~ (is_val l) /\ exists t', trans l t t' /\ u ≅ t' >>= k) \/
+    (exists (x : X), trans (val x) t stuck /\ trans l (k x) u).
+Proof.
+  intros TR.
+  eapply trans_bind_inv_aux.
+  apply TR.
+  rewrite <- ctree_eta; reflexivity.
+  rewrite <- ctree_eta; reflexivity.
+Qed.
+
+Lemma trans_bind_inv_l {X Y} `{Encode E} (t : ctree E X)
+  (k : X -> ctree E Y) (u : ctree E Y) l :
+  trans l (t >>= k) u ->
+  exists l' t', trans l' t t'.
+Proof.
+  intros TR.
+  apply trans_bind_inv in TR.
+  destruct TR as [(? & ? & ? & ?) | (? & ? & ?)]; eauto.
+Qed.
+
+(* Why this is needed? *)
+Local Typeclasses Transparent equ.
+Lemma trans_bind_l {X Y} `{HE: Encode E} (t : ctree E X)
+  (k : X -> ctree E Y) (u : ctree E X) (l: label E) :
+  ~ (is_val l) ->
+  trans l t u ->
+  trans l (t >>= k) (u >>= k).
+Proof.
+  cbn; unfold trans; intros NOV TR.
+  dependent induction TR; cbn in *.
+  - rewrite unfold_bind, <- x.
+    cbn.
+    econstructor.
+    now apply IHTR.
+  - rewrite unfold_bind.
+    rewrite <- x1; cbn.
+    econstructor.
+    rewrite H.
+    rewrite (ctree_eta t0),x,<- ctree_eta.
+    reflexivity.
+  - rewrite unfold_bind.
+    rewrite <- x1; cbn.
+    econstructor.
+    rewrite H.
+    rewrite (ctree_eta t0),x,<- ctree_eta.
+    reflexivity.
+  - exfalso; eapply NOV; constructor.
+Qed.
+
+Lemma trans_bind_r {X Y} `{HE: Encode E} (t : ctree E X)
+  (k : X -> ctree E Y) (u : ctree E Y) x l :
+  trans (val x) t stuck ->
+  trans l (k x) u ->
+  trans l (t >>= k) u.
+Proof.
+  cbn; unfold trans; intros TR1.
+  remember (observe stuck) as oc.
+  remember (val x) as v.
+  remember (observe t) as T.
+  generalize dependent t.
+  revert Heqv.
+  revert x Heqoc l u k.
+  induction TR1; intros; try (inv Heqv; fail).
+  - rewrite (ctree_eta t0), <- HeqT; cbn; econstructor.
+    eapply IHTR1; eauto.
+  - dependent induction Heqv.
+    rewrite (ctree_eta t0), <- HeqT, unfold_bind; cbn; auto.
+Qed.
+
+Lemma trans_val_invT {R R'} `{HE: Encode E}:
+  forall (t u : ctree E R) (v : R'),
+    trans (val v) t u ->
+    R = R'.
+Proof.
+  intros * TR.
+  remember (val v) as ov.
+  induction TR; intros; auto; try now inv Heqov.
+Qed.
+
+Lemma trans_trigger : forall {Y} `{HE: Encode E} (e : E) x (k: encode e -> ctree E Y),
+    trans (obs e x) (trigger e >>= k) (k x).
+Proof.
+  intros.
+  unfold Ctree.trigger.
+  rewrite unfold_bind; cbn.
+  setoid_rewrite bind_ret_l.
+  constructor; auto.
+Qed.
+
+Lemma trans_trigger_inv : forall {Y} `{HE: Encode E} (e : E)
+                            (k : encode e -> ctree E Y) l u,
+    trans l (trigger e >>= k) u ->
+    exists x, u ≅ k x /\ l = obs e x.
+Proof.
+  intros * TR.
+  unfold trigger in TR.
+  apply trans_bind_inv in TR.
+  destruct TR as [(? & ? & TR & ?) |(? & TR & ?)].
+  - apply trans_vis_inv in TR.
+    destruct TR as (? & ? & ->); eexists; split; eauto.
+    rewrite H0, H1, bind_ret_l; reflexivity.
+  - apply trans_vis_inv in TR.
+    destruct TR as (? & ? & abs); inv abs.
+Qed.
+
+(*| [wf_val] states that a [label] is well-formed:
+  if it is a [val] it should be of the right type. |*)
+Definition wf_val `{Encode E} X l :=
+  forall Y (v : Y), l = @val E _ Y v -> X = Y.
+
+Lemma wf_val_val `{Encode E} X (v : X):
+  wf_val X (@val E _ X v).
+Proof.
+  red. intros.
+  dependent destruction H0.
+  reflexivity.
+Qed.
+
+Lemma wf_val_nonval `{Encode E} X (l : label E):
+  ~is_val l -> wf_val X l.
+Proof.
+  red. intros. subst. exfalso. apply H0. constructor.
+Qed.
+
+Lemma wf_val_trans `{Encode E} {X} (l: label E)
+  (t t': ctree E X) :
+  trans l t t' -> wf_val X l.
+Proof.
+  red. intros. subst.
+  now apply trans_val_invT in H0.
+Qed.
+
+#[global] Hint Resolve
+ trans_ret trans_vis trans_br trans_guard
+ trans_br2_l trans_br2_r
+ trans_step trans_trigger trans_bind_l trans_bind_r: trans.
+
+#[global] Hint Constructors is_val : trans.
+#[global] Hint Resolve
+  wf_val_val wf_val_nonval wf_val_trans : trans.
+
+Ltac etrans := eauto with trans.
+
+Tactic Notation "trans" "in" ident(TR) :=
+  match type of TR with
+  | trans ?x (Ret ?r) ?u =>
+      let x' := fresh "x" in
+      let Eql := fresh "Eql" in
+      apply trans_ret_inv in TR as (x' & Eql); rewrite ?Eql in *
+  | trans (val ?x) ?t ?u =>
+      let Eqt := fresh "Eqt" in
+      rewrite ?(trans_val_invT TR) in *;
+      apply trans_val_inv in TR as Eqt
+  | trans ?l (Guard ?t) ?u =>
+      apply trans_guard_inv in TR
+  | trans ?l (step ?t) ?u =>
+      let Eqt := fresh "Eqt" in
+      let Eql := fresh "Eql" in
+      apply trans_step_inv in TR as (Eqt & Eql); rewrite ?Eql in *
+  | trans ?l (br2 ?t ?u) ?v =>
+      let Eqt := fresh "Eqt" in
+      let Eql := fresh "Eql" in
+      apply trans_br2_inv in TR as (Eql & [Eqt | Eqt]); rewrite ?Eql in *
+  | trans ?l (br3 ?t ?u ?v) ?t' =>
+      let Eqt := fresh "Eqt" in
+      let Eql := fresh "Eql" in
+      apply trans_br3_inv in TR as (Eql & [Eqt | [ Eqt | Equt ]]);
+      rewrite ?Eql in *
+  | trans ?l (Vis ?e ?k) ?u =>
+      let x := fresh "x" in
+      let Eqt := fresh "Eqt" in
+      let Eql := fresh "Eql" in
+      apply trans_vis_inv in TR as (x & Eqt & Eql); rewrite ?Eql in *
+  | trans ?l (x <- trigger ?e ;; ?k ?x) ?u =>
+      let x := fresh "x" in
+      let Eql := fresh "Eql" in
+      let Eqt := fresh "Eqt" in
+      apply trans_trigger_inv in TR as (x & Eqt & Eql); rewrite ?Eql in *
+  | trans ?l (Br ?n ?k) ?t =>
+      let n := fresh "n" in
+      let Eqt := fresh "Eqt" in
+      let Eql := fresh "Eql" in
+      apply trans_br_inv in TR as (n & Eqt & Eql); rewrite ?Eql in *
+  end.
